commit

ap/defs.lean
@@ -18,32 +18,32 @@ def dist (p₁ p₂ : Point) : ℕ :=
 
 structure Board : Type :=
 (squares : set Point)
-(angel : Point)
+(A : Point)
 
 def board₀ : Board := ⟨set.univ, center⟩
 
 -- Move
 
-def Angel_move : Type := Point
-def Devil_move : Type := option Point
+def A_move : Type := Point
+def D_move : Type := option Point
 
-def angel_move_valid (pw : ℕ) (b : Board) (p : Angel_move) : Prop :=
-p ≠ b.angel ∧ dist p b.angel ≤ pw ∧ p ∈ b.squares
+def A_move_valid (pw : ℕ) (b : Board) (p : A_move) : Prop :=
+p ≠ b.A ∧ dist p b.A ≤ pw ∧ p ∈ b.squares
 
-def devil_move_valid (b : Board) : Devil_move → Prop
+def D_move_valid (b : Board) : D_move → Prop
 | (option.none) := true
-| (option.some p) := p ≠ b.angel ∧ p ∈ b.squares
+| (option.some p) := p ≠ b.A ∧ p ∈ b.squares
 
-structure Valid_angel_move (pw : ℕ) (b : Board) :=
-(m : Angel_move)
-(h : angel_move_valid pw b m)
+structure Valid_A_move (pw : ℕ) (b : Board) :=
+(m : A_move)
+(h : A_move_valid pw b m)
 
-structure Valid_devil_move (b : Board) :=
-(m : Devil_move)
-(h : devil_move_valid b m)
+structure Valid_D_move (b : Board) :=
+(m : D_move)
+(h : D_move_valid b m)
 
-def angel_has_valid_move (pw : ℕ) (b : Board) :=
-∃ (m : Angel_move), angel_move_valid pw b m
+def A_has_valid_move (pw : ℕ) (b : Board) :=
+∃ (m : A_move), A_move_valid pw b m
 
 -- State
 
@@ -65,34 +65,34 @@ def State.finish (s : State) : State :=
 
 -- Player
 
-structure Angel (pw : ℕ) : Type :=
+structure A (pw : ℕ) : Type :=
 (f : Π (s : State), s.act →
-  angel_has_valid_move pw s.board → Valid_angel_move pw s.board)
+  A_has_valid_move pw s.board → Valid_A_move pw s.board)
 
-structure Devil : Type :=
-(f : Π (s : State), s.act → Valid_devil_move s.board)
+structure D : Type :=
+(f : Π (s : State), s.act → Valid_D_move s.board)
 
 def apply_move (s : State) (b : Board) : State :=
 {s with board := b, history := s.history ++ [s.board] }
 
-def apply_angel_move (s : State) (p : Angel_move) : State :=
-apply_move s {s.board with angel := p}
+def apply_A_move (s : State) (p : A_move) : State :=
+apply_move s {s.board with A := p}
 
-def apply_devil_move' (s : State) : Devil_move → Board
+def apply_D_move' (s : State) : D_move → Board
 | (option.none) := s.board
 | (option.some p) := {s.board with squares := s.board.squares \ {p}}
 
-def apply_devil_move (s : State) (m : Devil_move) : State :=
-apply_move s (apply_devil_move' s m)
+def apply_D_move (s : State) (m : D_move) : State :=
+apply_move s (apply_D_move' s m)
 
 -- Game
 
 @[ext] structure Game (pw : ℕ) : Type :=
-(a : Angel pw)
-(d : Devil)
+(a : A pw)
+(d : D)
 (s : State)
 
-def init_game {pw : ℕ} (a : Angel pw) (d : Devil) (s : State) : Game pw :=
+def init_game {pw : ℕ} (a : A pw) (d : D) (s : State) : Game pw :=
 { a := a, d := d, s := s }
 
 def Game.act {pw : ℕ} (g : Game pw) : Prop :=
@@ -101,32 +101,32 @@ g.s.act
 def Game.set_state {pw : ℕ} (g : Game pw) (s₁ : State) : Game pw :=
 {g with s := s₁}
 
-def play_angel_move_at' {pw pw₁ : ℕ} (a₁ : Angel pw₁) (g : Game pw) (hs h) :=
-g.set_state (apply_angel_move g.s (a₁.f g.s hs h).m)
+def play_A_move_at' {pw pw₁ : ℕ} (a₁ : A pw₁) (g : Game pw) (hs h) :=
+g.set_state (apply_A_move g.s (a₁.f g.s hs h).m)
 
 def Game.finish {pw : ℕ} (g : Game pw) : Game pw :=
 g.set_state g.s.finish
 
-def play_angel_move_at {pw : ℕ} (g : Game pw) :=
-if h : g.act ∧ angel_has_valid_move pw g.s.board
-then play_angel_move_at' g.a g h.1 h.2
+def play_A_move_at {pw : ℕ} (g : Game pw) :=
+if h : g.act ∧ A_has_valid_move pw g.s.board
+then play_A_move_at' g.a g h.1 h.2
 else g.finish
 
-def play_devil_move_at {pw : ℕ} (g : Game pw) (hs) :=
-g.set_state (apply_devil_move g.s (g.d.f g.s hs).m)
+def play_D_move_at {pw : ℕ} (g : Game pw) (hs) :=
+g.set_state (apply_D_move g.s (g.d.f g.s hs).m)
 
 def Game.play_move {pw : ℕ} (g : Game pw) :=
 if hs : g.act
-then play_angel_move_at (play_devil_move_at g hs)
+then play_A_move_at (play_D_move_at g hs)
 else g
 
 def Game.play {pw : ℕ} (g : Game pw) (n : ℕ) :=
 (Game.play_move^[n]) g
 
-def Game.angel_wins {pw : ℕ} (g : Game pw) :=
+def Game.A_wins {pw : ℕ} (g : Game pw) :=
 ∀ (n : ℕ), (g.play n).act
 
-def angel_hws_at (pw : ℕ) (s : State) :=
-∃ (a : Angel pw), ∀ (d : Devil), (init_game a d s).angel_wins
+def A_hws_at (pw : ℕ) (s : State) :=
+∃ (a : A pw), ∀ (d : D), (init_game a d s).A_wins
 
-def angel_hws (pw : ℕ) := angel_hws_at pw state₀
+def A_hws (pw : ℕ) := A_hws_at pw state₀
