ap/determinacy.lean
@@ -3,91 +3,91 @@ import data.int.basic
 import data.set.basic
 import logic.function.iterate
 
-import .defs .game
+import .defs .game .played_move
 
 noncomputable theory
 open_locale classical
 
-lemma not_angel_hws_at_of {pw : ℕ} {s : State}
-  (h : devil_hws_at pw s) : ¬angel_hws_at pw s :=
+lemma not_A_hws_at_of {pw : ℕ} {s : State}
+  (h : D_hws_at pw s) : ¬A_hws_at pw s :=
 begin
   cases h with d h, change ¬∃ _, _, push_neg,
-  intro a, use d, rw not_angel_wins_at, apply h,
+  intro a, use d, rw not_A_wins_at, apply h,
 end
 
-lemma not_devil_hws_at_of {pw : ℕ} {s : State}
-  (h : angel_hws_at pw s) : ¬devil_hws_at pw s :=
+lemma not_D_hws_at_of {pw : ℕ} {s : State}
+  (h : A_hws_at pw s) : ¬D_hws_at pw s :=
 begin
   cases h with d h, change ¬∃ _, _, push_neg,
-  intro a, use d, rw not_devil_wins_at, apply h,
+  intro a, use d, rw not_D_wins_at, apply h,
 end
 
 -----
 
-lemma act_of_not_devil_hws {pw : ℕ} {s : State}
-  (h : ¬devil_hws_at pw s) : s.act :=
+lemma act_of_not_D_hws {pw : ℕ} {s : State}
+  (h : ¬D_hws_at pw s) : s.act :=
 by { contrapose! h, use default, intro a, use 0 }
 
-lemma angel_hvm_of_not_devil_hws {pw : ℕ} {s : State}
-  (h : ¬devil_hws_at pw s) :
-  ∀ (md : Valid_devil_move s.board),
-  angel_has_valid_move pw (apply_devil_move s md.m).board :=
+lemma A_hvm_of_not_D_hws {pw : ℕ} {s : State}
+  (h : ¬D_hws_at pw s) :
+  ∀ (md : Valid_D_move s.board),
+  A_has_valid_move pw (apply_D_move s md.m).board :=
 begin
-  intro md, rw devil_hws_at at h, push_neg at h,
-  let d := (default : Devil).set_move s md, specialize h d,
-  cases h with a h, rw not_devil_wins_at at h, specialize h 1, rw play_1 at h,
+  intro md, rw D_hws_at at h, push_neg at h,
+  let d := (default : D).set_move s md, specialize h d,
+  cases h with a h, rw not_D_wins_at at h, specialize h 1, rw play_1 at h,
   rw Game.play_move at h, split_ifs at h with h₁, swap, { contradiction }, 
-  rw play_angel_move_at at h, split_ifs at h with h₂, swap, { cases h },
+  rw play_A_move_at at h, split_ifs at h with h₂, swap, { cases h },
   cases h₂ with h₂ h₃, convert h₃, change _ = dite _ _ _, rw dif_pos; refl,
 end
 
-lemma exi_moves_hws_of_not_devil_hws {pw : ℕ} {s : State}
-  (h : ¬devil_hws_at pw s) :
-  ∀ (md : Valid_devil_move s.board) (d : Devil),
-  ∃ (ma : Valid_angel_move pw (apply_devil_move s md.m).board) (a : Angel pw),
-  (init_game a d (apply_angel_move (apply_devil_move s md.m) ma.m)).angel_wins :=
+lemma exi_moves_hws_of_not_D_hws {pw : ℕ} {s : State}
+  (h : ¬D_hws_at pw s) :
+  ∀ (md : Valid_D_move s.board) (d : D),
+  ∃ (ma : Valid_A_move pw (apply_D_move s md.m).board) (a : A pw),
+  (init_game a d (apply_A_move (apply_D_move s md.m) ma.m)).A_wins :=
 begin
-  have hs : s.act := act_of_not_devil_hws h,
+  have hs : s.act := act_of_not_D_hws h,
   have h₁ : ¬∃ _, _ := h, push_neg at h₁,
-  simp_rw not_devil_wins_at at h₁, rintro md d₀, let md₀ := d₀.f s hs,
-  let d := d₀.set_move s md, let s' := apply_devil_move s md.m,
-  change apply_devil_move s md.m with s',
-  have h₂ : angel_has_valid_move pw s'.board,
-  { apply angel_hvm_of_not_devil_hws h },
+  simp_rw not_D_wins_at at h₁, rintro md d₀, let md₀ := d₀.f s hs,
+  let d := d₀.set_move s md, let s' := apply_D_move s md.m,
+  change apply_D_move s md.m with s',
+  have h₂ : A_has_valid_move pw s'.board,
+  { apply A_hvm_of_not_D_hws h },
   specialize h₁ d, cases h₁ with a h₁, let ma := a.f s' hs h₂, use [ma, a],
   have hh : d₀ = d.set_move s md₀,
   { change d₀ = (d₀.set_move s md).set_move s md₀,
-    rw [devil_set_move_set_move_eq, devil_set_move_self] },
-  rw hh, have h₃ : (init_game a d (apply_angel_move s' ma.m)).angel_wins,
-  { convert angel_wins_at_play_move_of h₁,
+    rw [D_set_move_set_move_eq, D_set_move_self] },
+  rw hh, have h₃ : (init_game a d (apply_A_move s' ma.m)).A_wins,
+  { convert A_wins_at_play_move_of h₁,
     rw init_game_play_move hs, change _ = dite _ _ _,
-    have h₃ : (play_devil_move_at (init_game a d s) hs).s = s',
-    { change apply_devil_move s _ = apply_devil_move s _,
+    have h₃ : (play_D_move_at (init_game a d s) hs).s = s',
+    { change apply_D_move s _ = apply_D_move s _,
       congr, change dite _ _ _ = md, change (init_game a d s).s with s,
       rw dif_pos rfl },
     simp_rw h₃, rw dif_pos, swap, { split; assumption },
-    ext; try {refl}, rw play_angel_move_at', dsimp,
-    simp_rw h₃, change (play_devil_move_at (init_game a d s) hs).a with a,
-    generalize_proofs h₄, convert_to _ = apply_angel_move s' (a.f s' hs h₂).m,
+    ext; try {refl}, rw play_A_move_at', dsimp,
+    simp_rw h₃, change (play_D_move_at (init_game a d s) hs).a with a,
+    generalize_proofs h₄, convert_to _ = apply_A_move s' (a.f s' hs h₂).m,
     { simp_rw Game.set_state, congr; try {exact h₃}, convert_to trivial == trivial,
       { exact eq_true_intro h₄ }, { exact eq_true_intro h₂ }, refl }, refl },
-  let g : Game pw := _, change g.angel_wins at h₃,
-  let g₁ : Game pw := _, change g₁.angel_wins,
-  have h₄ : g₁ = g.set_devil (d.set_move s md₀) := rfl, rw h₄, clear h₄,
-  have h₄ : s.len < (g.set_devil d).s.len,
+  let g : Game pw := _, change g.A_wins at h₃,
+  let g₁ : Game pw := _, change g₁.A_wins,
+  have h₄ : g₁ = g.set_D (d.set_move s md₀) := rfl, rw h₄, clear h₄,
+  have h₄ : s.len < (g.set_D d).s.len,
   { exact length_lt_length_snoc₂ },
-  apply (devil_set_move_angel_wins_iff h₄).mpr, exact h₃,
+  apply (D_set_move_A_wins_iff h₄).mpr, exact h₃,
 end
 
-def mk_devil_st_for_ma_exi_devil_st {pw : ℕ} {s' : State}
-  (h : ∀ (ma : Valid_angel_move pw s'.board),
-    ∃ (d : Devil), ∀ (a : Angel pw),
-    (init_game a d (apply_angel_move s' ma.m)).devil_wins) :
-  Devil :=
+def mk_D_st_for_ma_exi_D_st {pw : ℕ} {s' : State}
+  (h : ∀ (ma : Valid_A_move pw s'.board),
+    ∃ (d : D), ∀ (a : A pw),
+    (init_game a d (apply_A_move s' ma.m)).D_wins) :
+  D :=
 begin
   refine ⟨λ sx, _⟩,
-  apply dite (∃ (ma : Valid_angel_move pw s'.board),
-    angel_played_move_at sx s' ma); rintro h₁,
+  apply dite (∃ (ma : Valid_A_move pw s'.board),
+    A_played_move_at sx s' ma); rintro h₁,
   { exact (h h₁.some).some.f sx },
   { exact default },
 end
@@ -95,120 +95,120 @@ end
 -- Lemma 3.1.1
 -- Ross Bryant - Borel determinacy and metamathematics
 -- Master's thesis, University of North Texas, 2001
-lemma exi_angel_move_hws_of_not_devil_hws {pw : ℕ} {s : State}
-  (h : ¬devil_hws_at pw s) :
-  ∀ (md : Valid_devil_move s.board),
-  ∃ (ma : Valid_angel_move pw (apply_devil_move s md.m).board),
-  ¬devil_hws_at pw (apply_angel_move (apply_devil_move s md.m) ma.m) :=
+lemma exi_A_move_hws_of_not_D_hws {pw : ℕ} {s : State}
+  (h : ¬D_hws_at pw s) :
+  ∀ (md : Valid_D_move s.board),
+  ∃ (ma : Valid_A_move pw (apply_D_move s md.m).board),
+  ¬D_hws_at pw (apply_A_move (apply_D_move s md.m) ma.m) :=
 begin
-  have hs := act_of_not_devil_hws h,
-  have h₁ := exi_moves_hws_of_not_devil_hws h,
-  intro md, specialize h₁ md, simp_rw devil_hws_at, contrapose! h₁,
-  simp_rw not_angel_wins_at at h₁ ⊢,
-  let D := mk_devil_st_for_ma_exi_devil_st h₁, use D,
-  rintro ma a, have h₂ := h₁ ma, let s' := apply_devil_move s md.m,
-  change apply_devil_move s md.m with s' at ma h₁ h₂ ⊢,
-  let s₁ := apply_angel_move s' ma.m,
-  change apply_angel_move s' ma.m with s₁ at h₁ h₂ ⊢,
+  have hs := act_of_not_D_hws h,
+  have h₁ := exi_moves_hws_of_not_D_hws h,
+  intro md, specialize h₁ md, simp_rw D_hws_at, contrapose! h₁,
+  simp_rw not_A_wins_at at h₁ ⊢,
+  let D := mk_D_st_for_ma_exi_D_st h₁, use D,
+  rintro ma a, have h₂ := h₁ ma, let s' := apply_D_move s md.m,
+  change apply_D_move s md.m with s' at ma h₁ h₂ ⊢,
+  let s₁ := apply_A_move s' ma.m,
+  change apply_A_move s' ma.m with s₁ at h₁ h₂ ⊢,
   let d := h₂.some, have h₃ := h₂.some_spec,
-  change ∀ (a : Angel pw), (init_game a d s₁).devil_wins at h₃,
-  specialize h₃ a, contrapose! h₃, rw not_devil_wins_at at h₃ ⊢,
+  change ∀ (a : A pw), (init_game a d s₁).D_wins at h₃,
+  specialize h₃ a, contrapose! h₃, rw not_D_wins_at at h₃ ⊢,
   intro n, specialize h₃ n, suffices h₄ : (init_game a D s₁).play n =
-    ((init_game a d s₁).play n).set_devil D, { rwa h₄ at h₃ }, clear h₃,
+    ((init_game a d s₁).play n).set_D D, { rwa h₄ at h₃ }, clear h₃,
   induction n with n ih, { refl }, simp_rw [play_at_succ', ih], clear ih,
   let g : Game pw := _, change (init_game a d s₁).play n with g,
-  simp_rw Game.play_move, change (g.set_devil D).act with g.act,
+  simp_rw Game.play_move, change (g.set_D D).act with g.act,
   split_ifs with h₃, swap, { refl }, have h₅ : g.d = d := play_at_players_eq.2,
-  simp_rw play_devil_move_at, change (g.set_devil D).s with g.s,
-  change (g.set_devil D).d with D, rw h₅,
-  suffices h₆ : apply_devil_move g.s (D.f g.s h₃).m =
-    apply_devil_move g.s (d.f g.s h₃).m,
-  { rw [h₆, ←play_angel_move_at_set_devil], refl },
-  simp_rw apply_devil_move, congr' 3,
-  have h₆ : ∃ (ma : Valid_angel_move pw s'.board),
-    angel_played_move_at g.s s' ma,
-  { exact ⟨_, angel_played_move_at_play
-    (angel_played_move_at_apply_move hs rfl)⟩ },
-  change (mk_devil_st_for_ma_exi_devil_st _).f _ _ = _,
-  rw mk_devil_st_for_ma_exi_devil_st, dsimp,
+  simp_rw play_D_move_at, change (g.set_D D).s with g.s,
+  change (g.set_D D).d with D, rw h₅,
+  suffices h₆ : apply_D_move g.s (D.f g.s h₃).m =
+    apply_D_move g.s (d.f g.s h₃).m,
+  { rw [h₆, ←play_A_move_at_set_D], refl },
+  simp_rw apply_D_move, congr' 3,
+  have h₆ : ∃ (ma : Valid_A_move pw s'.board),
+    A_played_move_at g.s s' ma,
+  { exact ⟨_, A_played_move_at_play
+    (A_played_move_at_apply_move hs rfl)⟩ },
+  change (mk_D_st_for_ma_exi_D_st _).f _ _ = _,
+  rw mk_D_st_for_ma_exi_D_st, dsimp,
   split_ifs with hx, swap, { contradiction }, clear hx,
-  generalize_proofs h₇, change apply_devil_move s md.m with s' at h₇,
+  generalize_proofs h₇, change apply_D_move s md.m with s' at h₇,
   have h₈ := h₇.some_spec, change d with h₂.some, congr,
-  suffices h₉ : apply_angel_move (apply_devil_move s md.m) h₆.some.m = s₁,
-  { rw h₉ }, change apply_angel_move s' _ = apply_angel_move _ _, congr,
-  apply angel_played_move_at_eq h₆.some_spec,
-  exact angel_played_move_at_play (angel_played_move_at_apply_move hs rfl),
+  suffices h₉ : apply_A_move (apply_D_move s md.m) h₆.some.m = s₁,
+  { rw h₉ }, change apply_A_move s' _ = apply_A_move _ _, congr,
+  apply A_played_move_at_eq h₆.some_spec,
+  exact A_played_move_at_play (A_played_move_at_apply_move hs rfl),
 end
 
-def mk_angel_st_for_not_devil_hws (pw : ℕ) : Angel pw :=
+def mk_A_st_for_not_D_hws (pw : ℕ) : A pw :=
 begin
   refine ⟨λ s' h, _⟩,
-  apply dite (∃ (s : State) (md : Valid_devil_move s.board),
-    ¬devil_hws_at pw s ∧ s' = apply_devil_move s md.m); rintro h₁ h₂,
-  { refine (_ : ∃ (ma : Valid_angel_move pw s'.board),
-      ¬devil_hws_at pw (apply_angel_move s' ma.m)).some,
+  apply dite (∃ (s : State) (md : Valid_D_move s.board),
+    ¬D_hws_at pw s ∧ s' = apply_D_move s md.m); rintro h₁ h₂,
+  { refine (_ : ∃ (ma : Valid_A_move pw s'.board),
+      ¬D_hws_at pw (apply_A_move s' ma.m)).some,
     rcases h₁ with ⟨s, md, h₁, rfl⟩,
-    use (exi_angel_move_hws_of_not_devil_hws h₁ _).some,
+    use (exi_A_move_hws_of_not_D_hws h₁ _).some,
     generalize_proofs h₂, exact h₂.some_spec },
   { exact ⟨_, h₂.some_spec⟩ },
 end
 
-lemma not_devil_hws_at_play_of_not_devil_hws {pw n : ℕ} {g : Game pw}
-  (h₁ : g.a = mk_angel_st_for_not_devil_hws pw)
-  (h₂ : ¬devil_hws_at pw g.s) :
-  ¬devil_hws_at pw (g.play n).s :=
+lemma not_D_hws_at_play_of_not_D_hws {pw n : ℕ} {g : Game pw}
+  (h₁ : g.a = mk_A_st_for_not_D_hws pw)
+  (h₂ : ¬D_hws_at pw g.s) :
+  ¬D_hws_at pw (g.play n).s :=
 begin
   rename g g₀, induction n with n ih, { exact h₂ }, clear h₂,
   rw play_at_succ', let g : Game pw := _,
-  change ¬devil_hws_at pw g.s at ih,
-  change ¬devil_hws_at pw g.play_move.s,
+  change ¬D_hws_at pw g.s at ih,
+  change ¬D_hws_at pw g.play_move.s,
   change g.play_move with dite _ _ _,
   split_ifs, swap, { exact ih },
   let d := g.d, let s := g.s, let md := d.f s h,
-  let s' := apply_devil_move s md.m,
-  have h₃ : ∃ (ma : Valid_angel_move pw s'.board),
-    ¬devil_hws_at pw (apply_angel_move s' ma.m),
-  { exact exi_angel_move_hws_of_not_devil_hws ih md },
+  let s' := apply_D_move s md.m,
+  have h₃ : ∃ (ma : Valid_A_move pw s'.board),
+    ¬D_hws_at pw (apply_A_move s' ma.m),
+  { exact exi_A_move_hws_of_not_D_hws ih md },
   have ma := h₃.some, have h₄ := h₃.some_spec,
   convert h₄, change Game.s (dite _ _ _) = _,
-  have h₅ : angel_has_valid_move pw s'.board := ⟨_, ma.h⟩,
-  change (play_devil_move_at g h).s with s',
+  have h₅ : A_has_valid_move pw s'.board := ⟨_, ma.h⟩,
+  change (play_D_move_at g h).s with s',
   rw dif_pos, swap, { split; assumption },
-  change apply_angel_move _ _ = _, congr,
-  change g.a.f s' h h₅ = _, let A : Angel pw := _, change g₀.a = A at h₁,
+  change apply_A_move _ _ = _, congr,
+  change g.a.f s' h h₅ = _, let A : A pw := _, change g₀.a = A at h₁,
   have h₆ : g.a = A := by { rw ←h₁, exact play_at_players_eq.1 },
-  rw h₆, change (mk_angel_st_for_not_devil_hws pw).f _ _ _ = _,
-  rw mk_angel_st_for_not_devil_hws, dsimp, rw dif_pos, exact ⟨s, md, ih, rfl⟩,
+  rw h₆, change (mk_A_st_for_not_D_hws pw).f _ _ _ = _,
+  rw mk_A_st_for_not_D_hws, dsimp, rw dif_pos, exact ⟨s, md, ih, rfl⟩,
 end
 
-lemma angel_hws_at_of {pw : ℕ} {s : State}
-  (h : ¬devil_hws_at pw s) : angel_hws_at pw s :=
+lemma A_hws_at_of {pw : ℕ} {s : State}
+  (h : ¬D_hws_at pw s) : A_hws_at pw s :=
 begin
-  have hs : s.act := act_of_not_devil_hws h,
-  let A := mk_angel_st_for_not_devil_hws pw, use A, rintro d n,
+  have hs : s.act := act_of_not_D_hws h,
+  let A := mk_A_st_for_not_D_hws pw, use A, rintro d n,
   induction n with n ih, { exact hs }, rw play_at_succ',
   let g : Game pw := _, change g.act at ih, change g.play_move.act,
-  let s := g.s, let md := d.f s ih, let s' := apply_devil_move s md.m,
-  rw play_move_at_act ih, have h₁ : play_devil_move_at g ih = g.set_state s',
-  { convert play_devil_move_eq, change apply_devil_move _ (d.f s ih).m = _,
+  let s := g.s, let md := d.f s ih, let s' := apply_D_move s md.m,
+  rw play_move_at_act ih, have h₁ : play_D_move_at g ih = g.set_state s',
+  { convert play_D_move_eq, change apply_D_move _ (d.f s ih).m = _,
     congr, symmetry, exact play_at_players_eq.2 },
-  rw h₁, clear h₁, have h₁ : angel_has_valid_move pw s'.board,
-  { have h₁ : ¬devil_hws_at pw s := not_devil_hws_at_play_of_not_devil_hws rfl h,
-    exact ⟨_, (exi_angel_move_hws_of_not_devil_hws h₁ md).some.h⟩ },
+  rw h₁, clear h₁, have h₁ : A_has_valid_move pw s'.board,
+  { have h₁ : ¬D_hws_at pw s := not_D_hws_at_play_of_not_D_hws rfl h,
+    exact ⟨_, (exi_A_move_hws_of_not_D_hws h₁ md).some.h⟩ },
   change Game.act (dite _ _ _), change (g.set_state s').s with s',
   rw dif_pos, swap, { split; assumption }, exact ih,
 end
 
 -----
 
-lemma devil_hws_at_of {pw : ℕ} {s : State}
-  (h : ¬angel_hws_at pw s) : devil_hws_at pw s :=
-by { contrapose! h, exact angel_hws_at_of h }
+lemma D_hws_at_of {pw : ℕ} {s : State}
+  (h : ¬A_hws_at pw s) : D_hws_at pw s :=
+by { contrapose! h, exact A_hws_at_of h }
 
-lemma not_angel_hws_at_iff {pw : ℕ} {s : State} :
-  ¬angel_hws_at pw s ↔ devil_hws_at pw s :=
-⟨devil_hws_at_of, not_angel_hws_at_of⟩
+lemma not_A_hws_at_iff {pw : ℕ} {s : State} :
+  ¬A_hws_at pw s ↔ D_hws_at pw s :=
+⟨D_hws_at_of, not_A_hws_at_of⟩
 
-lemma not_devil_hws_at_iff {pw : ℕ} {s : State} :
-  ¬devil_hws_at pw s ↔ angel_hws_at pw s :=
-⟨angel_hws_at_of, not_devil_hws_at_of⟩
+lemma not_D_hws_at_iff {pw : ℕ} {s : State} :
+  ¬D_hws_at pw s ↔ A_hws_at pw s :=
+⟨A_hws_at_of, not_D_hws_at_of⟩
