ap/game.lean
@@ -10,45 +10,36 @@ import .base .point .dist .board .state .player
 noncomputable theory
 open_locale classical
 
-def Game.set_angel {pw pw₁ : ℕ} (g : Game pw) (a₁ : Angel pw₁) : Game pw₁ :=
+def Game.set_A {pw pw₁ : ℕ} (g : Game pw) (a₁ : A pw₁) : Game pw₁ :=
 {g with a := a₁}
 
-def Game.set_devil {pw : ℕ} (g : Game pw) (d₁ : Devil) : Game pw :=
+def Game.set_D {pw : ℕ} (g : Game pw) (d₁ : D) : Game pw :=
 {g with d := d₁}
 
 def Game.set_players {pw pw₁ : ℕ} (g : Game pw)
-  (a₁ : Angel pw₁) (d₁ : Devil) : Game pw₁ :=
-(g.set_angel a₁).set_devil d₁
+  (a₁ : A pw₁) (d₁ : D) : Game pw₁ :=
+(g.set_A a₁).set_D d₁
 
 def Game.set_prev_moves {pw : ℕ} (g : Game pw)
-  (fa : Angel_prev_moves pw g.s)
-  (fd : Devil_prev_moves g.s) : Game pw :=
+  (fa : A_prev_moves pw g.s)
+  (fd : D_prev_moves g.s) : Game pw :=
 g.set_players (g.a.set_prev_moves g.s fa) (g.d.set_prev_moves g.s fd)
 
-def Game.devil_wins {pw : ℕ} (g : Game pw) :=
+def Game.D_wins {pw : ℕ} (g : Game pw) :=
 ∃ (n : ℕ), ¬(g.play n).act
 
-def devil_hws_at (pw : ℕ) (s : State) :=
-∃ (d : Devil), ∀ (a : Angel pw), (init_game a d s).devil_wins
-
-def angel_played_move_at {pw : ℕ} (s : State) (s₀' : State)
-  (ma : Valid_angel_move pw s₀'.board) : Prop :=
-∃ (s₀ : State) (md : Valid_devil_move s₀.board) (a : Angel pw) (d : Devil) (n : ℕ),
-(∃ hs, d.f s₀ hs = md) ∧
-s₀' = apply_devil_move s₀ md.m ∧
-(∃ hs h, a.f s₀' hs h = ma) ∧
-n ≠ 0 ∧
-s = ((init_game a d s₀).play n).s
+def D_hws_at (pw : ℕ) (s : State) :=
+∃ (d : D), ∀ (a : A pw), (init_game a d s).D_wins
 
 -----
 
-lemma not_angel_wins_at {pw : ℕ} {g : Game pw} :
-  ¬g.angel_wins ↔ g.devil_wins :=
-by simp [Game.angel_wins, Game.devil_wins]
+lemma not_A_wins_at {pw : ℕ} {g : Game pw} :
+  ¬g.A_wins ↔ g.D_wins :=
+by simp [Game.A_wins, Game.D_wins]
 
-lemma not_devil_wins_at {pw : ℕ} {g : Game pw} :
-  ¬g.devil_wins ↔ g.angel_wins :=
-by simp [Game.angel_wins, Game.devil_wins]
+lemma not_D_wins_at {pw : ℕ} {g : Game pw} :
+  ¬g.D_wins ↔ g.A_wins :=
+by simp [Game.A_wins, Game.D_wins]
 
 lemma play_at_succ {pw n : ℕ} {g : Game pw} :
   g.play n.succ = g.play_move.play n :=
@@ -60,38 +51,38 @@ function.iterate_succ_apply' _ _ _
 
 -----
 
-lemma angel_wins_at_play_of {pw : ℕ} {g : Game pw}
-  (h : g.angel_wins) {n : ℕ} : (g.play n).angel_wins :=
+lemma A_wins_at_play_of {pw : ℕ} {g : Game pw}
+  (h : g.A_wins) {n : ℕ} : (g.play n).A_wins :=
 begin
   intro k, specialize h (k + n),
   rw [Game.play, function.iterate_add] at h, exact h,
 end
 
-lemma angel_wins_at_play_move_of {pw : ℕ} {g : Game pw}
-  (h : g.angel_wins) : g.play_move.angel_wins :=
-@angel_wins_at_play_of _ _ h 1
+lemma A_wins_at_play_move_of {pw : ℕ} {g : Game pw}
+  (h : g.A_wins) : g.play_move.A_wins :=
+@A_wins_at_play_of _ _ h 1
 
-lemma play_angel_move_at_players_eq {pw : ℕ} {g : Game pw} :
-  (play_angel_move_at g).a = g.a ∧ (play_angel_move_at g).d = g.d :=
-by { rw [play_angel_move_at], split_ifs; exact ⟨rfl, rfl⟩ }
+lemma play_A_move_at_players_eq {pw : ℕ} {g : Game pw} :
+  (play_A_move_at g).a = g.a ∧ (play_A_move_at g).d = g.d :=
+by { rw [play_A_move_at], split_ifs; exact ⟨rfl, rfl⟩ }
 
-lemma play_devil_move_at_players_eq {pw : ℕ} {g : Game pw} {hs} :
-  (play_devil_move_at g hs).a = g.a ∧ (play_devil_move_at g hs).d = g.d :=
-by { rw [play_devil_move_at], exact ⟨rfl, rfl⟩ }
+lemma play_D_move_at_players_eq {pw : ℕ} {g : Game pw} {hs} :
+  (play_D_move_at g hs).a = g.a ∧ (play_D_move_at g hs).d = g.d :=
+by { rw [play_D_move_at], exact ⟨rfl, rfl⟩ }
 
 lemma play_move_at_players_eq {pw : ℕ} {g : Game pw} :
   g.play_move.a = g.a ∧ g.play_move.d = g.d :=
 begin
   rw [Game.play_move], split_ifs, swap, exact ⟨rfl, rfl⟩,
-  rw [play_angel_move_at_players_eq.1, play_angel_move_at_players_eq.2],
-  rw [play_devil_move_at_players_eq.1, play_devil_move_at_players_eq.2],
+  rw [play_A_move_at_players_eq.1, play_A_move_at_players_eq.2],
+  rw [play_D_move_at_players_eq.1, play_D_move_at_players_eq.2],
   exact ⟨rfl, rfl⟩,
 end
 
 lemma play_move_at_players_eq' {pw : ℕ} {g : Game pw} {hs} :
-  (play_angel_move_at (play_devil_move_at g hs)).a = g.a ∧
-  (play_angel_move_at (play_devil_move_at g hs)).d = g.d :=
-by { rw play_angel_move_at, split_ifs; exact ⟨rfl, rfl⟩ }
+  (play_A_move_at (play_D_move_at g hs)).a = g.a ∧
+  (play_A_move_at (play_D_move_at g hs)).d = g.d :=
+by { rw play_A_move_at, split_ifs; exact ⟨rfl, rfl⟩ }
 
 lemma play_at_players_eq {pw n : ℕ} {g : Game pw} :
   (g.play n).a = g.a ∧ (g.play n).d = g.d :=
@@ -104,7 +95,7 @@ end
 
 lemma play_move_at_act {pw : ℕ} {g : Game pw}
   (h : g.act) :
-  g.play_move = play_angel_move_at (play_devil_move_at g h) :=
+  g.play_move = play_A_move_at (play_D_move_at g h) :=
 dif_pos h
 
 lemma play_move_at_not_act {pw : ℕ} {g : Game pw}
@@ -112,28 +103,28 @@ lemma play_move_at_not_act {pw : ℕ} {g : Game pw}
   g.play_move = g :=
 dif_neg h
 
-lemma play_angel_move_hvm {pw : ℕ} {g : Game pw} (hs)
-  (h : angel_has_valid_move pw g.s.board) :
-  ∃ h, play_angel_move_at g = play_angel_move_at' g.a g hs h :=
+lemma play_A_move_hvm {pw : ℕ} {g : Game pw} (hs)
+  (h : A_has_valid_move pw g.s.board) :
+  ∃ h, play_A_move_at g = play_A_move_at' g.a g hs h :=
 by exact ⟨_, dif_pos ⟨hs, h⟩⟩
 
-lemma play_angel_move_at_set_devil {pw : ℕ}
-  {g : Game pw} {d₁ : Devil} :
-  play_angel_move_at (g.set_devil d₁) = (play_angel_move_at g).set_devil d₁ :=
-by { simp_rw play_angel_move_at, split_ifs; refl }
+lemma play_A_move_at_set_D {pw : ℕ}
+  {g : Game pw} {d₁ : D} :
+  play_A_move_at (g.set_D d₁) = (play_A_move_at g).set_D d₁ :=
+by { simp_rw play_A_move_at, split_ifs; refl }
 
-lemma play_devil_move_at_set_angel {pw pw₁ : ℕ}
-  {g : Game pw} {a₁ : Angel pw₁} {hs} :
-  play_devil_move_at (g.set_angel a₁) hs =
-  (play_devil_move_at g hs).set_angel a₁ :=
+lemma play_D_move_at_set_A {pw pw₁ : ℕ}
+  {g : Game pw} {a₁ : A pw₁} {hs} :
+  play_D_move_at (g.set_A a₁) hs =
+  (play_D_move_at g hs).set_A a₁ :=
 rfl
 
-lemma angel_has_valid_move_at_play_devil_move {pw : ℕ} {g : Game pw} {hs}
-  (h : g.angel_wins) :
-  angel_has_valid_move pw (play_devil_move_at g hs).s.board :=
+lemma A_has_valid_move_at_play_D_move {pw : ℕ} {g : Game pw} {hs}
+  (h : g.A_wins) :
+  A_has_valid_move pw (play_D_move_at g hs).s.board :=
 begin
   specialize h 1, change g.play_move.act at h,
-  rw play_move_at_act hs at h, rw play_angel_move_at at h,
+  rw play_move_at_act hs at h, rw play_A_move_at at h,
   split_ifs at h with h₁,
   { exact h₁.2 },
   { cases h },
@@ -157,43 +148,43 @@ begin
   { rw play_at_succ' at h₂, exact ih (act_play_move_at_succ h₂) },
 end
 
-lemma hist_len_play_angel_move_at' {pw pw₁ : ℕ} {g : Game pw}
-  {a₁ : Angel pw₁} {h₁ h₂} :
-  (play_angel_move_at' a₁ g h₁ h₂).s.len = g.s.len.succ :=
-hist_len_apply_angel_move
+lemma hist_len_play_A_move_at' {pw pw₁ : ℕ} {g : Game pw}
+  {a₁ : A pw₁} {h₁ h₂} :
+  (play_A_move_at' a₁ g h₁ h₂).s.len = g.s.len.succ :=
+hist_len_apply_A_move
 
-lemma hist_len_play_devil_move_at {pw : ℕ} {g : Game pw} {hs} :
-  (play_devil_move_at g hs).s.len = g.s.len.succ :=
-hist_len_apply_devil_move
+lemma hist_len_play_D_move_at {pw : ℕ} {g : Game pw} {hs} :
+  (play_D_move_at g hs).s.len = g.s.len.succ :=
+hist_len_apply_D_move
 
-lemma play_angel_move_at_hist_len_ge {pw : ℕ} {g : Game pw} :
-  g.s.len ≤ (play_angel_move_at g).s.len :=
+lemma play_A_move_at_hist_len_ge {pw : ℕ} {g : Game pw} :
+  g.s.len ≤ (play_A_move_at g).s.len :=
 begin
-  rw play_angel_move_at, split_ifs, swap, { refl },
-  rw hist_len_play_angel_move_at',
+  rw play_A_move_at, split_ifs, swap, { refl },
+  rw hist_len_play_A_move_at',
   exact nat.le_of_lt (nat.lt_succ_self _),
 end
 
-lemma play_devil_move_at_hist_len_ge {pw : ℕ} {g : Game pw} {hs} :
-  g.s.len ≤ (play_devil_move_at g hs).s.len :=
-by { rw hist_len_play_devil_move_at, exact nat.le_of_lt (nat.lt_succ_self _) }
+lemma play_D_move_at_hist_len_ge {pw : ℕ} {g : Game pw} {hs} :
+  g.s.len ≤ (play_D_move_at g hs).s.len :=
+by { rw hist_len_play_D_move_at, exact nat.le_of_lt (nat.lt_succ_self _) }
 
-lemma play_devil_move_at_hist_len_eq {pw : ℕ} {g : Game pw} {hs} :
-  (play_devil_move_at g hs).s.len = g.s.len.succ :=
-by rw hist_len_play_devil_move_at
+lemma play_D_move_at_hist_len_eq {pw : ℕ} {g : Game pw} {hs} :
+  (play_D_move_at g hs).s.len = g.s.len.succ :=
+by rw hist_len_play_D_move_at
 
 lemma play_move_at_hist_len_ge {pw : ℕ} {g : Game pw} :
   g.s.len ≤ g.play_move.s.len :=
 begin
   rw Game.play_move, split_ifs with hs, swap, { refl },
-  rw play_angel_move_at, split_ifs with h₁,
-  { change (play_devil_move_at g hs).a with g.a,
-    transitivity (play_devil_move_at g hs).s.len,
-    { exact play_devil_move_at_hist_len_ge },
-    { rw hist_len_play_angel_move_at',
+  rw play_A_move_at, split_ifs with h₁,
+  { change (play_D_move_at g hs).a with g.a,
+    transitivity (play_D_move_at g hs).s.len,
+    { exact play_D_move_at_hist_len_ge },
+    { rw hist_len_play_A_move_at',
       exact nat.le_of_lt (nat.lt_succ_self _) }},
-  { change _ ≤ (play_devil_move_at g hs).s.len,
-    rw hist_len_play_devil_move_at,
+  { change _ ≤ (play_D_move_at g hs).s.len,
+    rw hist_len_play_D_move_at,
     exact nat.le_of_lt (nat.lt_succ_self _) },
 end
 
@@ -207,8 +198,8 @@ begin
 end
 
 lemma set_players_flip {pw pw₁ : ℕ} {g : Game pw}
-  {a₁ : Angel pw₁} {d₁ : Devil} :
-  (g.set_angel a₁).set_devil d₁ = (g.set_devil d₁).set_angel a₁ :=
+  {a₁ : A pw₁} {d₁ : D} :
+  (g.set_A a₁).set_D d₁ = (g.set_D d₁).set_A a₁ :=
 rfl
 
 lemma play_move_eq_set_state_of_act_next {pw : ℕ} {g : Game pw}
@@ -221,17 +212,17 @@ begin
   { refl },
 end
 
-lemma play_devil_move_eq {pw : ℕ} {g : Game pw} {hs} :
-  play_devil_move_at g hs =
-  g.set_state (apply_devil_move g.s (g.d.f g.s hs).m) :=
+lemma play_D_move_eq {pw : ℕ} {g : Game pw} {hs} :
+  play_D_move_at g hs =
+  g.set_state (apply_D_move g.s (g.d.f g.s hs).m) :=
 rfl
 
 -----
 
-lemma set_prev_moves_angel_wins_iff {pw : ℕ} {g : Game pw}
-  {fa : Angel_prev_moves pw g.s}
-  {fd : Devil_prev_moves g.s} :
-  (g.set_prev_moves fa fd).angel_wins ↔ g.angel_wins :=
+lemma set_prev_moves_A_wins_iff {pw : ℕ} {g : Game pw}
+  {fa : A_prev_moves pw g.s}
+  {fd : D_prev_moves g.s} :
+  (g.set_prev_moves fa fd).A_wins ↔ g.A_wins :=
 begin
   let a := g.a, let d := g.d,
   let a' := a.set_prev_moves g.s fa,
@@ -246,15 +237,15 @@ begin
   change (g₁.set_players a' d').play_move = g₁.play_move.set_players a' d',
   simp_rw Game.play_move,
   split_ifs, swap, { refl },
-  have h₁ : play_devil_move_at (g₁.set_players a' d') h =
-    (play_devil_move_at g₁ h).set_players a' d',
-  { simp_rw [Game.set_players, set_players_flip, play_devil_move_at_set_angel],
-    congr, simp_rw play_devil_move_at,
-    change (g₁.set_devil d').d with d',
-    ext; try { refl }, change _ = apply_devil_move _ _,
-    simp [apply_devil_move, apply_move], simp_rw Game.set_state,
+  have h₁ : play_D_move_at (g₁.set_players a' d') h =
+    (play_D_move_at g₁ h).set_players a' d',
+  { simp_rw [Game.set_players, set_players_flip, play_D_move_at_set_A],
+    congr, simp_rw play_D_move_at,
+    change (g₁.set_D d').d with d',
+    ext; try { refl }, change _ = apply_D_move _ _,
+    simp [apply_D_move, apply_move], simp_rw Game.set_state,
     refine ⟨_, snoc_eq_snoc_iff.mpr ⟨rfl, rfl⟩, rfl⟩,
-    change (g₁.set_devil d').s with g₁.s,
+    change (g₁.set_D d').s with g₁.s,
     congr' 1, generalize_proofs, change d'.f g₁.s h with dite _ _ _,
     split_ifs with h₂,
     { exfalso, contrapose! h₂, clear h₂,
@@ -263,49 +254,49 @@ begin
       { refl }},
     { congr, exact play_at_players_eq.2.symm }},
   rw h₁, clear h₁,
-  let g₂ : Game pw := _, change (play_devil_move_at g₁ h) with g₂,
-  have h₁ : play_angel_move_at (g₂.set_angel a') =
-    (play_angel_move_at g₂).set_angel a',
-  { simp_rw play_angel_move_at,
-    change dite (g₂.act ∧ angel_has_valid_move pw g₂.s.board) _ _ = _,
+  let g₂ : Game pw := _, change (play_D_move_at g₁ h) with g₂,
+  have h₁ : play_A_move_at (g₂.set_A a') =
+    (play_A_move_at g₂).set_A a',
+  { simp_rw play_A_move_at,
+    change dite (g₂.act ∧ A_has_valid_move pw g₂.s.board) _ _ = _,
     split_ifs with hx, swap, { refl },
-    change (g₂.set_angel a').a with a',
-    simp_rw play_angel_move_at', ext; try {refl},
+    change (g₂.set_A a').a with a',
+    simp_rw play_A_move_at', ext; try {refl},
     simp_rw Game.set_state,
-    change (g₂.set_angel a').s with g₂.s at hx ⊢,
-    change _ = apply_angel_move _ _,
-    simp [apply_angel_move, apply_move],
+    change (g₂.set_A a').s with g₂.s at hx ⊢,
+    change _ = apply_A_move _ _,
+    simp [apply_A_move, apply_move],
     generalize_proofs hy hz,
     change a'.f g₂.s h hy with dite _ _ _,
     split_ifs with h₂,
     { exfalso, contrapose! h₂, clear h₂,
       transitivity (g.play n).s.len,
       { exact play_at_hist_len_ge },
-      { exact play_devil_move_at_hist_len_ge }},
+      { exact play_D_move_at_hist_len_ge }},
     { congr, exact play_at_players_eq.1.symm }},
-  simp_rw [Game.set_players, play_angel_move_at_set_devil, h₁],
+  simp_rw [Game.set_players, play_A_move_at_set_D, h₁],
 end
 
-lemma angel_set_move_angel_wins_iff {pw : ℕ} {g : Game pw}
-  {s : State} {m : Valid_angel_move pw s.board}
+lemma A_set_move_A_wins_iff {pw : ℕ} {g : Game pw}
+  {s : State} {m : Valid_A_move pw s.board}
   (h : s.len < g.s.len) :
-  (g.set_angel (g.a.set_move s m)).angel_wins ↔ g.angel_wins :=
+  (g.set_A (g.a.set_move s m)).A_wins ↔ g.A_wins :=
 begin
-  convert set_prev_moves_angel_wins_iff, ext,
-  { change _ = g.a.prev_moves_set g.s s m h, rw angel_prev_moves_set_eq, refl },
+  convert set_prev_moves_A_wins_iff, ext,
+  { change _ = g.a.prev_moves_set g.s s m h, rw A_prev_moves_set_eq, refl },
   repeat { refl }, change _ = g.d.prev_moves_id g.s,
-  rw devil_prev_moves_id_eq, refl,
+  rw D_prev_moves_id_eq, refl,
 end
 
-lemma devil_set_move_angel_wins_iff {pw : ℕ} {g : Game pw}
-  {s : State} {m : Valid_devil_move s.board}
+lemma D_set_move_A_wins_iff {pw : ℕ} {g : Game pw}
+  {s : State} {m : Valid_D_move s.board}
   (h : s.len < g.s.len) :
-  (g.set_devil (g.d.set_move s m)).angel_wins ↔ g.angel_wins :=
+  (g.set_D (g.d.set_move s m)).A_wins ↔ g.A_wins :=
 begin
-  convert set_prev_moves_angel_wins_iff, ext,
-  { change _ = g.a.prev_moves_id g.s, rw angel_prev_moves_id_eq, },
+  convert set_prev_moves_A_wins_iff, ext,
+  { change _ = g.a.prev_moves_id g.s, rw A_prev_moves_id_eq, },
   repeat { refl }, change _ = g.d.prev_moves_set g.s s m h,
-  rw devil_prev_moves_set_eq,
+  rw D_prev_moves_set_eq,
 end
 
 lemma play_1 {pw : ℕ} {g : Game pw} : g.play 1 = g.play_move := rfl
@@ -313,237 +304,15 @@ lemma play_1 {pw : ℕ} {g : Game pw} : g.play 1 = g.play_move := rfl
 -----
 
 lemma init_game_act {pw : ℕ}
-  {a : Angel pw} {d : Devil} {s : State}
+  {a : A pw} {d : D} {s : State}
   (h : s.act) :
   (init_game a d s).act := h
 
 lemma init_game_play_move {pw : ℕ}
-  {a : Angel pw} {d : Devil} {s : State} (hs) :
+  {a : A pw} {d : D} {s : State} (hs) :
   (init_game a d s).play_move =
-  play_angel_move_at (play_devil_move_at (init_game a d s) hs) :=
+  play_A_move_at (play_D_move_at (init_game a d s) hs) :=
 dif_pos (init_game_act hs)
-
-lemma angel_played_move_at_apply_move {pw : ℕ} {s s' : State}
-  {md : Valid_devil_move s.board} {ma : Valid_angel_move pw s'.board}
-  (hs : s.act) (h : s' = apply_devil_move s md.m) :
-  angel_played_move_at (apply_angel_move s' ma.m) s' ma :=
-begin
-  let a := (default : Angel pw).set_move s' ma,
-  let d := (default : Devil).set_move s md,
-  use [s, md, a, d, 1, ⟨hs, devil_set_move_eq_pos⟩, h],
-  have hs₁ : s'.act := by rwa h,
-  have hvm_s' : angel_has_valid_move pw s'.board := ⟨_, ma.h⟩,
-  refine ⟨_, _, _⟩, { exact ⟨hs₁, hvm_s', angel_set_move_eq_pos⟩ },
-  { dec_trivial }, rw [play_1, play_move_at_act], swap, { exact hs },
-  rw play_angel_move_at, rw dif_pos, swap,
-  { use hs, convert hvm_s', convert h.symm,
-    change apply_devil_move s (d.f s hs).m = _, congr,
-    exact devil_set_move_eq_pos },
-  symmetry, change apply_angel_move _ _ = _,
-  have h₁ : (play_devil_move_at (init_game a d s) hs).s = s',
-  { convert h.symm, change apply_devil_move s (d.f s hs).m = _,
-    congr, exact devil_set_move_eq_pos },
-  congr' 1, change (a.f _ _ _).m = _, generalize_proofs h₂,
-  have h₃ : (a.f (play_devil_move_at (init_game a d s) hs).s hs h₂).m =
-    (a.f s' hs₁ hvm_s').m, { congr' },
-  rw [h₃, angel_set_move_eq_pos],
-end
-
-lemma angel_hvm_of_next_act {pw : ℕ} {g : Game pw}
-  (h : g.play_move.act) :
-  ∃ hs, angel_has_valid_move pw (play_devil_move_at g hs).s.board :=
-begin
-  have hs : g.act := act_play_move_at_succ h, use hs,
-  rw Game.play_move at h, rw dif_pos hs at h,
-  rw play_angel_move_at at h, split_ifs at h with h₄,
-  { cases h₄ with h₄ h₅, convert h₅, },
-  { cases h }
-end
-
-lemma play_move_hist_len_eq_of_act {pw : ℕ} {g : Game pw}
-  (h : g.play_move.act) :
-  g.play_move.s.len = g.s.len + 2 :=
-begin
-  have h₁ : g.act := act_play_move_at_succ h,
-  rw [play_move_at_act h₁, play_angel_move_at],
-  rw dif_pos, { rw [hist_len_play_angel_move_at', hist_len_play_devil_move_at] },
-  exact ⟨h₁, (angel_hvm_of_next_act h).some_spec⟩,
-end
-
-lemma play_hist_len_eq_of_act {pw n : ℕ} {g : Game pw}
-  (h : (g.play n).act) :
-  (g.play n).s.len = g.s.len + n * 2 :=
-begin
-  induction n with n ih, { refl }, rw play_at_succ' at h ⊢,
-  let g₁ : Game pw := _, change g.play n with g₁ at ih h ⊢,
-  have h₁ := act_play_move_at_succ h, specialize ih h₁,
-  rw [play_move_hist_len_eq_of_act h, ih, add_assoc, nat.succ_mul],
-end
-
-lemma hist_len_ne_of_play_lt {pw n k : ℕ} {g : Game pw}
-  (h₁ : k < n) (h₂ : (g.play n).act) :
-  (g.play k).s.len ≠ (g.play n).s.len :=
-begin
-  have h₃ := act_play_at_le (nat.le_of_lt h₁) h₂,
-  rw [play_hist_len_eq_of_act h₂, play_hist_len_eq_of_act h₃], intro h,
-  replace h := nat.add_left_cancel h,
-  rw nat.mul_left_inj at h, swap, { dec_trivial },
-  subst h, exact nat.lt_asymm h₁ h₁,
-end
-
-lemma hist_ne_of_play_lt {pw n k : ℕ} {g : Game pw}
-  (h₁ : k < n) (h₂ : (g.play n).act) :
-  (g.play k).s.history ≠ (g.play n).s.history :=
-hist_ne_of_hist_len_ne (hist_len_ne_of_play_lt h₁ h₂)
-
-lemma state_ne_of_play_lt {pw n k : ℕ} {g : Game pw}
-  (h₁ : k < n) (h₂ : (g.play n).act) :
-  (g.play k).s ≠ (g.play n).s :=
-by { have h₃ := hist_ne_of_play_lt h₁ h₂, contrapose! h₃, rw h₃ }
-
-lemma apply_angel_move_ne_of_hist_ne {pw : ℕ} {s₁ s₂ : State}
-  {ma₁ ma₂ : Angel_move} (h : s₁.len ≠ s₂.len) :
-  apply_angel_move s₁ ma₁ ≠ apply_angel_move s₂ ma₂ :=
-begin
-  contrapose! h, simp_rw [apply_angel_move, apply_move] at h,
-  simp_rw [State.len, (snoc_eq_snoc_iff.mp h.2.1).1],
-end
-
-lemma apply_devil_move_ne_of_hist_ne {s₁ s₂ : State}
-  {md₁ md₂ : Devil_move} (h : s₁.len ≠ s₂.len) :
-  apply_devil_move s₁ md₁ ≠ apply_devil_move s₂ md₂ :=
-begin
-  contrapose! h, simp_rw [apply_devil_move, apply_move] at h,
-  simp_rw [State.len, (snoc_eq_snoc_iff.mp h.2.1).1],
-end
-
-def mk_angel_for_played_move_at_play_move {pw : ℕ}
-  (a₀ a : Angel pw) (s' : State) (hs : s'.act) :
-  Angel pw :=
-if hvm : angel_has_valid_move pw s'.board
-then a₀.set_move s' (a.f s' hs hvm)
-else a₀
-
-lemma angel_played_move_at_play_move {pw : ℕ}
-  {g : Game pw} {s₀' : State} {ma : Valid_angel_move pw s₀'.board}
-  (h : angel_played_move_at g.s s₀' ma) :
-  angel_played_move_at g.play_move.s s₀' ma :=
-begin
-  let a := g.a, let d := g.d, let s := g.s,
-  rcases h with ⟨s₀, md₀, a₀, d₀, n, hmd, h₁, hx, hy, h₂⟩, by_cases hs : g.act,
-  { let md := d.f s hs, let s' := apply_devil_move s md.m,
-    let d₁ := d₀.set_move s md,
-    let a₁ := mk_angel_for_played_move_at_play_move a₀ a s' hs,
-    have hmd₁ : ∃ hs, d₁.f s₀ hs = md₀,
-    { cases hmd with hs₁ hmd, use hs₁, change dite _ _ _ = _,
-      rw dif_neg, { exact hmd }, change ((init_game a₀ d₀ s₀).play 0).s ≠ g.s,
-      rw h₂, apply state_ne_of_play_lt (nat.pos_of_ne_zero hy),
-      change g.s.act at hs, rwa h₂ at hs },
-    use [s₀, md₀, a₁, d₁, n.succ, hmd₁, by rw h₁],
-    have h₁ : ∀ (k ≤ n), ((init_game a₁ d₁ s₀).play k).s =
-      ((init_game a₀ d₀ s₀).play k).s,
-    { rintro k hk, induction k with k ih, { refl }, simp_rw play_at_succ',
-      specialize ih (nat.le_of_succ_le hk),
-      replace ih : (init_game a₁ d₁ s₀).play k =
-        ((init_game a₀ d₀ s₀).play k).set_players a₁ d₁,
-      { ext,
-        { exact play_at_players_eq.1 },
-        { exact play_at_players_eq.2 },
-        { rw ih, refl }},
-      rw ih, clear ih,
-      have hs₁ : ((init_game a₀ d₀ s₀).play k).act,
-      { apply act_play_at_le (nat.le_of_succ_le hk),
-        change ((init_game a₀ d₀ s₀).play n).s.act,
-        rw ←h₂, exact hs },
-      repeat { rw play_move_at_act, swap, { exact hs₁ }},
-      let g₁ : Game pw := _,
-      change (init_game a₀ d₀ s₀).play k with g₁ at hs₁ ⊢,
-      have ha : g₁.a = a₀ := play_at_players_eq.1,
-      have hd : g₁.d = d₀ := play_at_players_eq.2,
-      let sk := g₁.s, let mdk := d₀.f sk hs₁,
-      let sk' := apply_devil_move sk mdk.m,
-      have hy : (play_devil_move_at g₁ hs₁).s = sk',
-      { change apply_devil_move sk _ = apply_devil_move _ _, congr' 2, rw hd },
-      have h₁ : d₁.f sk hs₁ = mdk,
-      { change dite _ _ _ = _, rw dif_neg,
-        change ((init_game a₀ d₀ s₀).play k).s ≠ g.s, rw h₂,
-        apply state_ne_of_play_lt (nat.succ_le_iff.mp hk),
-        change ((init_game a₀ d₀ s₀).play n).s.act, rw ←h₂, exact hs },
-      have hx : play_devil_move_at (g₁.set_players a₁ d₁) hs₁ =
-        (play_devil_move_at g₁ hs₁).set_players a₁ d₁,
-      { ext,
-        { exact play_devil_move_at_players_eq.1, },
-        { exact play_devil_move_at_players_eq.2, },
-        { change apply_devil_move g₁.s _ = apply_devil_move _ _,
-          congr' 2, change d₁.f sk _ = _, rw [h₁, hd] }},
-      rw hx, clear hx, have hx : angel_has_valid_move pw sk'.board,
-      { have h₃ : g₁.play_move.act,
-        { change ((init_game a₀ d₀ s₀).play k).play_move.act,
-          rw ←play_at_succ', apply act_play_at_le hk,
-          change ((init_game a₀ d₀ s₀).play n).s.act,
-          rw ←h₂, exact hs },
-        convert (angel_hvm_of_next_act h₃).some_spec, rw ←hy, refl },
-      simp_rw play_angel_move_at,
-      repeat { rw dif_pos, swap, { use hs₁, convert hx }},
-      change apply_angel_move (play_devil_move_at g₁ hs₁).s
-        (a₁.f (play_devil_move_at g₁ hs₁).s _ _).m =
-        apply_angel_move _ (g₁.a.f (play_devil_move_at g₁ hs₁).s _ _).m,
-      congr' 2, rw ha, generalize_proofs h₃,
-      change (mk_angel_for_played_move_at_play_move _ _ _ _).f _ _ _ = _,
-      rw mk_angel_for_played_move_at_play_move,
-      split_ifs with hh, swap, { refl },
-      change dite _ _ _ = _, rw dif_neg, rw hy,
-      change apply_devil_move ((init_game a₀ d₀ s₀).play k).s mdk.m ≠
-        apply_devil_move g.s md.m,
-      rw h₂, replace hk := nat.lt_of_succ_le hk,
-      apply apply_devil_move_ne_of_hist_ne, apply hist_len_ne_of_play_lt hk,
-      change ((init_game a₀ d₀ s₀).play n).s.act, rw ←h₂, exact hs },
-    specialize h₁ n (le_refl n),
-    replace h₁ : (init_game a₁ d₁ s₀).play n = g.set_players a₁ d₁,
-    { ext,
-      { exact play_at_players_eq.1 },
-      { exact play_at_players_eq.2 },
-      { rw h₁, exact h₂.symm }},
-    rw [play_at_succ', play_move_at_act hs, h₁, play_move_at_act],
-    swap, { exact hs }, refine ⟨_, _, _⟩,
-    { clear h₁, rcases hx with ⟨hs', h, hx⟩,
-      use [hs', h], rw ←hx, clear hx,
-      change (mk_angel_for_played_move_at_play_move _ _ _ _).f _ _ _ = _,
-      rw mk_angel_for_played_move_at_play_move,
-      split_ifs with hss, swap, { refl }, change dite _ _ _ = _,
-      rw dif_neg, change s₀' ≠ apply_devil_move g.s _, rw [h₁, h₂],
-      apply apply_devil_move_ne_of_hist_ne,
-      change ((init_game a₀ d₀ s₀).play 0).s.len ≠ _,
-      apply hist_len_ne_of_play_lt (pos_iff_ne_zero.mpr hy),
-      rw [Game.act, ←h₂], exact hs }, { dec_trivial }, symmetry,
-    have h₁ : play_devil_move_at (g.set_players a₁ d₁) hs =
-      (play_devil_move_at g hs).set_players a₁ d₁,
-    { ext,
-      { exact play_devil_move_at_players_eq.1 },
-      { exact play_devil_move_at_players_eq.2 },
-      { change apply_devil_move g.s _ = apply_devil_move _ _,
-        congr' 2, change d₁.f s hs = g.d.f g.s hs,
-        change dite _ _ _ = _, rw dif_pos rfl }},
-    rw h₁, clear h₁, simp_rw play_angel_move_at,
-    split_ifs with h₁, swap, { refl }, cases h₁ with h₁ h₂,
-    change apply_angel_move ((play_devil_move_at g hs).s) _ =
-      apply_angel_move _ _,
-    congr' 2, change a₁.f s' _ _ = a.f s' _ _, generalize_proofs,
-    change (mk_angel_for_played_move_at_play_move _ _ _ _).f _ _ _ = _,
-    rw mk_angel_for_played_move_at_play_move, rw dif_pos, swap, { exact h₂ },
-    change dite _ _ _ = _, rw dif_pos rfl },
-  { use [s₀, md₀, a₀, d₀, n, hmd, h₁, hx, hy],
-    rw play_move_at_not_act hs, exact h₂ },
-end
-
-lemma angel_played_move_at_play {pw n : ℕ}
-  {g : Game pw} {s' : State} {ma : Valid_angel_move pw s'.board}
-  (h : angel_played_move_at g.s s' ma) :
-  angel_played_move_at (g.play n).s s' ma :=
-begin
-  induction n with n ih, { exact h }, rw play_at_succ',
-  exact angel_played_move_at_play_move ih,
-end
 
 lemma hist_len_game_finish {pw : ℕ} {g : Game pw} :
   g.finish.s.len = g.s.len := rfl
@@ -552,10 +321,10 @@ lemma hist_len_le_play_move {pw : ℕ} {g : Game pw} :
   g.s.len ≤ g.play_move.s.len :=
 begin
   rw Game.play_move, split_ifs with hs, swap, { refl },
-  rw play_angel_move_at, split_ifs with h,
-  { rw [hist_len_play_angel_move_at', hist_len_play_devil_move_at],
+  rw play_A_move_at, split_ifs with h,
+  { rw [hist_len_play_A_move_at', hist_len_play_D_move_at],
     apply nat.le_succ_of_le (nat.le_succ _) },
-  { rw [hist_len_game_finish, hist_len_play_devil_move_at],
+  { rw [hist_len_game_finish, hist_len_play_D_move_at],
     apply nat.le_succ },
 end
 
@@ -564,94 +333,4 @@ lemma hist_len_le_play {pw n : ℕ} {g : Game pw} :
 begin
   induction n with n ih, { refl }, rw play_at_succ',
   exact ih.trans hist_len_le_play_move,
-end
-
-lemma hist_overlaps_of_angel_played_move_at {pw : ℕ}
-  {s s₀' : State} {ma : Valid_angel_move pw s₀'.board}
-  (h₁ : angel_played_move_at s s₀' ma) :
-  ∀ (k : ℕ), k.succ < s₀'.len →
-  s.history.nth k = s₀'.history.nth k :=
-begin
-  rintro k h₂,
-  rcases h₁ with ⟨s₀, md, a, d, n, hmd, rfl, hx, hy, rfl⟩, clear' hx hy,
-  change (apply_devil_move s₀ md.m).history with (_ ++ _ : list _) at h₂ ⊢,
-  change _ < (snoc _ _).length at h₂,
-  rw [length_snoc, nat.succ_lt_succ_iff] at h₂ ,induction n with n ih,
-  { change s₀.history.nth k = _, exact (list.nth_append h₂).symm },
-  { simp_rw play_at_succ', let g : Game pw := _,
-    change (init_game a d s₀).play n with g at h₂ ih ⊢, rw ←ih, clear ih,
-    rw Game.play_move, split_ifs with hs, swap, { refl }, rw play_angel_move_at,
-    have h₆ : s₀.len ≤ g.s.len,
-    { change (init_game a d s₀).s.len ≤ _, exact hist_len_le_play },
-    split_ifs with h₃,
-    { change (_ ++ _ : list _).nth _ = _, rw list.nth_append,
-      { change (_ ++ _ : list _).nth _ = _, rw list.nth_append,
-        exact gt_of_ge_of_gt h₆ h₂ },
-      { rw [←State.len, hist_len_play_devil_move_at],
-        exact nat.lt_succ_of_le (nat.le_trans (le_of_lt h₂) h₆) }},
-    { change (_ ++ _ : list _).nth _ = _, rw list.nth_append,
-      exact gt_of_ge_of_gt h₆ h₂ }},
-end
-
-lemma angel_played_move_at_eq_aux {pw n : ℕ}
-  {sx s₀ s' : State} {md : Valid_devil_move s₀.board}
-  {a : Angel pw} {d : Devil} {hs hvm h₄}
-  (h₁ : s' = apply_devil_move s₀ md.m)
-  (h₂ : sx = ((init_game a d s₀).play n).s)
-  (h₃ : n ≠ 0)
-  (hh : md = d.f s₀ h₄) :
-  sx.nth (s₀.len + 2) = option.some
-    (apply_angel_move s' (a.f s' hs hvm).m).board :=
-begin
-  cases n, { contradiction }, clear h₃,
-  let i : ℕ := _, change s₀.len + 2 with i,
-  let s₁ : State := apply_angel_move s' (a.f s' hs hvm).m,
-  change _ = some (State.board s₁), have h₅ : i = s₁.len,
-  { change s₁ with apply_angel_move _ _, subst s',
-    rw [apply_angel_move_len, apply_devil_move_len] },
-  induction n with n ih generalizing sx,
-  { rw [play_1, play_move_at_act] at h₂, swap, { exact h₄ },
-    subst sx, have h₆ : play_devil_move_at (init_game a d s₀) h₄ =
-      (init_game a d s'),
-    { ext,
-      { exact play_devil_move_at_players_eq.1 },
-      { exact play_devil_move_at_players_eq.2 },
-      { subst s',
-        change apply_devil_move s₀ (d.f s₀ _).m = apply_devil_move s₀ _, rw hh }},
-    rw [h₆, play_angel_move_at, dif_pos], clear h₆, swap, { exact ⟨hs, hvm⟩ },
-    change s₁.nth _ = _, rw h₅, exact state_nth_len },
-  { rw play_at_succ' at h₂, let g₁ : Game pw := (init_game a d s₀).play n.succ,
-    change (init_game a d s₀).play n.succ with g₁ at ih h₂, subst sx,
-    specialize ih rfl, rw Game.play_move, split_ifs with hs₁, swap, { exact ih },
-    let g₂ : Game pw := _, change play_devil_move_at g₁ hs₁ with g₂,
-    have ih₁ : g₂.s.nth i = some s₁.board,
-    { exact apply_move_state_nth_eq_some_of ih },
-    rw play_angel_move_at, split_ifs with hh,
-    { exact apply_move_state_nth_eq_some_of ih₁ },
-    { exact ih₁ }},
-end
-
-lemma angel_played_move_at_eq {pw : ℕ}
-  {sx s' : State} {ma₁ ma₂ : Valid_angel_move pw s'.board}
-  (hx : angel_played_move_at sx s' ma₁)
-  (hy : angel_played_move_at sx s' ma₂) :
-  ma₁ = ma₂ :=
-begin
-  obtain ⟨s₀, md₁, a₁, d₁, n₁, hmd₁, h₁, ⟨hs₁, hvm₁, rfl⟩, h₃, h₄⟩ := hx,
-  obtain ⟨s₀', md₂, a₂, d₂, n₂, hmd₂, h₅, ⟨hs₂, hvm₂, rfl⟩, h₇, h₈⟩ := hy,
-  have hs : s₀.act,
-  { subst s', exact hs₂ },
-  obtain rfl : s₀ = s₀',
-  { subst h₁, exact state_eq_of_apply_devil_move_eq h₅ },
-  obtain rfl : md₁ = md₂,
-  { subst h₁, rwa ←devil_moves_eq_iff at h₅ },
-  clear h₅, change hvm₂ with hvm₁, clear hvm₂,
-  change hs₂ with hs₁, clear hs₂, let i := s₀.len,
-  have h₅ : sx.nth (i + 2) = option.some
-    (apply_angel_move s' (a₁.f s' hs₁ hvm₁).m).board,
-  { exact angel_played_move_at_eq_aux h₁ h₄ h₃ hmd₁.some_spec.symm },
-  have h₆ : sx.nth (i + 2) = option.some
-    (apply_angel_move s' (a₂.f s' hs₁ hvm₁).m).board,
-  { exact angel_played_move_at_eq_aux h₁ h₈ h₇ hmd₂.some_spec.symm },
-  simp [h₅] at h₆, rwa angel_moves_eq_iff',
 end
