ap/lemmas.lean
@@ -6,43 +6,43 @@ import .base .game .pw_ge
 noncomputable theory
 open_locale classical
 
-def play {pw : ℕ} (a : Angel pw) (d : Devil) (n : ℕ) :=
+def play {pw : ℕ} (a : A pw) (d : D) (n : ℕ) :=
 (init_game a d state₀).play n
 
-def angel_wins {pw : ℕ} (a : Angel pw) (d : Devil) :=
-(init_game a d state₀).angel_wins
+def A_wins {pw : ℕ} (a : A pw) (d : D) :=
+(init_game a d state₀).A_wins
 
-def devil_wins {pw : ℕ} (a : Angel pw) (d : Devil) :=
-(init_game a d state₀).devil_wins
+def D_wins {pw : ℕ} (a : A pw) (d : D) :=
+(init_game a d state₀).D_wins
 
-def devil_hws (pw : ℕ) := devil_hws_at pw state₀
+def D_hws (pw : ℕ) := D_hws_at pw state₀
 
 -----
 
-lemma angel_pw_0_not_hws : ¬angel_hws 0 :=
+lemma A_pw_0_not_hws : ¬A_hws 0 :=
 begin
-  rintro ⟨a, h⟩, contrapose! h, clear h, use default, rw not_angel_wins_at, use 1,
+  rintro ⟨a, h⟩, contrapose! h, clear h, use default, rw not_A_wins_at, use 1,
   rw [play_1, play_move_at_act], swap, { triv },
-  rw [play_angel_move_at, dif_neg], { exact not_false },
+  rw [play_A_move_at, dif_neg], { exact not_false },
   push_neg, rintro h₁ ⟨ma, h₂, h₃, h₄⟩,
   rw [nat.le_zero_iff, dist_eq_zero_iff] at h₃, contradiction,
 end
 
-lemma angel_pw_1_not_hws : ¬angel_hws 1 :=
+lemma A_pw_1_not_hws : ¬A_hws 1 :=
 begin
   sorry
 end
 
-lemma angel_pw_2_hws : angel_hws 2 :=
+lemma A_pw_2_hws : A_hws 2 :=
 begin
   sorry
 end
 
 -----
 
-lemma angel_pw_ge_hws {pw pw₁ : ℕ}
-  (h₁ : pw ≤ pw₁) (h₂ : angel_hws pw) : angel_hws pw₁ :=
+lemma A_pw_ge_hws {pw pw₁ : ℕ}
+  (h₁ : pw ≤ pw₁) (h₂ : A_hws pw) : A_hws pw₁ :=
 begin
-  cases h₂ with a h₂, use mk_angel_pw_ge a h₁,
-  intro d, specialize h₂ d, apply mk_angel_pw_ge_wins_at_of h₂,
+  cases h₂ with a h₂, use mk_A_pw_ge a h₁,
+  intro d, specialize h₂ d, apply mk_A_pw_ge_wins_at_of h₂,
 end
