ap/pw_ge.lean
@@ -7,88 +7,88 @@ import .base .player .game
 noncomputable theory
 open_locale classical
 
-def mk_angel_pw_ge {pw pw₁ : ℕ} (a : Angel pw)
-  (h₁ : pw ≤ pw₁) : Angel pw₁ :=
+def mk_A_pw_ge {pw pw₁ : ℕ} (a : A pw)
+  (h₁ : pw ≤ pw₁) : A pw₁ :=
 begin
   refine ⟨λ s hs h, _⟩,
-  refine dite (angel_has_valid_move pw s.board) (λ h₂, _) (λ h₂, _),
+  refine dite (A_has_valid_move pw s.board) (λ h₂, _) (λ h₂, _),
   { have v := a.f s hs h₂, refine ⟨v.1, v.2.1, v.2.2.1.trans h₁, v.2.2.2⟩ },
   { refine ⟨_, h.some_spec⟩ },
 end
 
-lemma sup_mk_angel_pw_ge {pw pw₁ : ℕ} {a : Angel pw}
+lemma sup_mk_A_pw_ge {pw pw₁ : ℕ} {a : A pw}
   {h : pw ≤ pw₁} :
-  (mk_angel_pw_ge a h).sup a :=
+  (mk_A_pw_ge a h).sup a :=
 begin
-  rintro s hs h₁, have h₂ := angel_has_valid_move_ge_of h h₁,
-  use [hs, h₂], simp_rw [mk_angel_pw_ge, dif_pos h₁],
+  rintro s hs h₁, have h₂ := A_has_valid_move_ge_of h h₁,
+  use [hs, h₂], simp_rw [mk_A_pw_ge, dif_pos h₁],
 end
 
-lemma angel_has_valid_move_of_exi_sub {pw pw₁ : ℕ}
-  {a₁ : Angel pw₁} {b : Board}
-  (h₁ : ∃ (a : Angel pw), a.sub a₁)
-  (h₂ : angel_has_valid_move pw b) :
-  angel_has_valid_move pw₁ b :=
+lemma A_has_valid_move_of_exi_sub {pw pw₁ : ℕ}
+  {a₁ : A pw₁} {b : Board}
+  (h₁ : ∃ (a : A pw), a.sub a₁)
+  (h₂ : A_has_valid_move pw b) :
+  A_has_valid_move pw₁ b :=
 (h₁.some_spec (init_state b) trivial ⟨_, h₂.some_spec⟩).some_spec.some
 
-lemma sup_angel_play_angel_move_at_eq {pw pw₁ pw₂ : ℕ}
-  {g : Game pw} {a₁ : Angel pw₁} {a₂ : Angel pw₂} {hs : g.act}
+lemma sup_A_play_A_move_at_eq {pw pw₁ pw₂ : ℕ}
+  {g : Game pw} {a₁ : A pw₁} {a₂ : A pw₂} {hs : g.act}
   (h₁ : a₂.sup a₁)
-  (h₂ : angel_has_valid_move pw₁ g.s.board) :
-  ∃ h₃, play_angel_move_at' a₂ g hs h₃ = play_angel_move_at' a₁ g hs h₂ :=
+  (h₂ : A_has_valid_move pw₁ g.s.board) :
+  ∃ h₃, play_A_move_at' a₂ g hs h₃ = play_A_move_at' a₁ g hs h₂ :=
 begin
   obtain ⟨hs, h₃, h₅⟩ := h₁ g.s hs h₂, use h₃,
-  simp_rw play_angel_move_at', congr',
+  simp_rw play_A_move_at', congr',
 end
 
-lemma sup_angel_play_eq {pw pw₁ n : ℕ}
-  {g : Game pw} {a₁ : Angel pw₁}
-  (h₁ : g.angel_wins)
+lemma sup_A_play_eq {pw pw₁ n : ℕ}
+  {g : Game pw} {a₁ : A pw₁}
+  (h₁ : g.A_wins)
   (h₂ : a₁.sup g.a) :
-  (g.set_angel a₁).play n = (g.play n).set_angel a₁ :=
+  (g.set_A a₁).play n = (g.play n).set_A a₁ :=
 begin
   let a := g.a, let d := g.d,
   induction n with n ih, { refl },
   simp_rw play_at_succ',
   rw ih, clear ih,
   let g₁ := _, change g.play n with g₁,
-  have wins_at_g₁ : g₁.angel_wins := angel_wins_at_play_of h₁,
-  have hvm_pw₁_of : ∀ {b : Board}, angel_has_valid_move pw b →
-    angel_has_valid_move pw₁ b := λ b, angel_has_valid_move_of_exi_sub ⟨_, h₂⟩,
+  have wins_at_g₁ : g₁.A_wins := A_wins_at_play_of h₁,
+  have hvm_pw₁_of : ∀ {b : Board}, A_has_valid_move pw b →
+    A_has_valid_move pw₁ b := λ b, A_has_valid_move_of_exi_sub ⟨_, h₂⟩,
   have act_g₁ : g₁.act := h₁ n,
-  have act_g₁_a₁ : (g₁.set_angel a₁).act := h₁ n,
+  have act_g₁_a₁ : (g₁.set_A a₁).act := h₁ n,
   rw play_move_at_act act_g₁,
   rw play_move_at_act act_g₁_a₁,
-  simp_rw play_devil_move_at_set_angel,
-  let g₂ := _, change play_devil_move_at g₁ act_g₁ with g₂,
-  have hvm_pw : angel_has_valid_move pw g₂.s.board,
-  { exact angel_has_valid_move_at_play_devil_move wins_at_g₁ },
-  have hvm_pw₁ : angel_has_valid_move pw₁ g₂.s.board,
+  simp_rw play_D_move_at_set_A,
+  let g₂ := _, change play_D_move_at g₁ act_g₁ with g₂,
+  have hvm_pw : A_has_valid_move pw g₂.s.board,
+  { exact A_has_valid_move_at_play_D_move wins_at_g₁ },
+  have hvm_pw₁ : A_has_valid_move pw₁ g₂.s.board,
   { exact hvm_pw₁_of hvm_pw },
-  have hvm_pw' : angel_has_valid_move pw (g₂.set_angel a₁).s.board,
+  have hvm_pw' : A_has_valid_move pw (g₂.set_A a₁).s.board,
   { exact hvm_pw },
-  have hvm_pw₁' : angel_has_valid_move pw₁ (g₂.set_angel a₁).s.board,
+  have hvm_pw₁' : A_has_valid_move pw₁ (g₂.set_A a₁).s.board,
   { exact hvm_pw₁ },
   have act_g₂ : g₂.act := act_g₁,
-  have act_g₂_a₁ : (g₂.set_angel a₁).act := act_g₂,
-  rw (play_angel_move_hvm act_g₂ hvm_pw).some_spec,
-  change play_angel_move_at (g₂.set_angel a₁) = _,
-  rw (play_angel_move_hvm act_g₂_a₁ hvm_pw₁').some_spec,
+  have act_g₂_a₁ : (g₂.set_A a₁).act := act_g₂,
+  rw (play_A_move_hvm act_g₂ hvm_pw).some_spec,
+  change play_A_move_at (g₂.set_A a₁) = _,
+  rw (play_A_move_hvm act_g₂_a₁ hvm_pw₁').some_spec,
   generalize_proofs,
-  change (g₂.set_angel a₁).a with a₁,
+  change (g₂.set_A a₁).a with a₁,
   have g₁_a_eq : g₁.a = a := play_at_players_eq.1,
   have g₂_a_eq : g₂.a = a,
   { convert_to g₂.a = g₁.a, { exact g₁_a_eq.symm },
-    exact play_devil_move_at_players_eq.1 },
+    exact play_D_move_at_players_eq.1 },
   rw g₂_a_eq,
-  have h₃ : play_angel_move_at' a₁ (g₂.set_angel a₁) act_g₂_a₁ hvm_pw₁ =
-    play_angel_move_at' a (g₂.set_angel a₁) act_g₂_a₁ hvm_pw',
-  { exact (sup_angel_play_angel_move_at_eq h₂ _).some_spec },
+  have h₃ : play_A_move_at' a₁ (g₂.set_A a₁) act_g₂_a₁ hvm_pw₁ =
+    play_A_move_at' a (g₂.set_A a₁) act_g₂_a₁ hvm_pw',
+  { exact (sup_A_play_A_move_at_eq h₂ _).some_spec },
   rw h₃, refl,
 end
 
-lemma mk_angel_pw_ge_wins_at_of {pw pw₁ : ℕ}
+lemma mk_A_pw_ge_wins_at_of {pw pw₁ : ℕ}
   {g : Game pw} {h₁ : pw ≤ pw₁}
-  (h₂ : g.angel_wins) :
-  (g.set_angel (mk_angel_pw_ge g.a h₁)).angel_wins :=
-by { intro n, rw (sup_angel_play_eq h₂) sup_mk_angel_pw_ge, exact h₂ n }
+  (h₂ : g.A_wins) :
+  (g.set_A (mk_A_pw_ge g.a h₁)).A_wins :=
+by { intro n, rw (sup_A_play_eq h₂) sup_mk_A_pw_ge, exact h₂ n }
