ap/played_move.lean
@@ -1,0 +1,334 @@
+import tactic
+import tactic.induction
+import data.int.basic
+import data.set.basic
+import logic.function.iterate
+import data.list
+
+import .base .game
+
+noncomputable theory
+open_locale classical
+
+def A_played_move_at {pw : ℕ} (s : State) (s₀' : State)
+  (ma : Valid_A_move pw s₀'.board) : Prop :=
+∃ (s₀ : State) (md : Valid_D_move s₀.board) (a : A pw) (d : D) (n : ℕ),
+(∃ hs, d.f s₀ hs = md) ∧
+s₀' = apply_D_move s₀ md.m ∧
+(∃ hs h, a.f s₀' hs h = ma) ∧
+n ≠ 0 ∧
+s = ((init_game a d s₀).play n).s
+
+-----
+
+lemma A_played_move_at_apply_move {pw : ℕ} {s s' : State}
+  {md : Valid_D_move s.board} {ma : Valid_A_move pw s'.board}
+  (hs : s.act) (h : s' = apply_D_move s md.m) :
+  A_played_move_at (apply_A_move s' ma.m) s' ma :=
+begin
+  let a := (default : A pw).set_move s' ma,
+  let d := (default : D).set_move s md,
+  use [s, md, a, d, 1, ⟨hs, D_set_move_eq_pos⟩, h],
+  have hs₁ : s'.act := by rwa h,
+  have hvm_s' : A_has_valid_move pw s'.board := ⟨_, ma.h⟩,
+  refine ⟨_, _, _⟩, { exact ⟨hs₁, hvm_s', A_set_move_eq_pos⟩ },
+  { dec_trivial }, rw [play_1, play_move_at_act], swap, { exact hs },
+  rw play_A_move_at, rw dif_pos, swap,
+  { use hs, convert hvm_s', convert h.symm,
+    change apply_D_move s (d.f s hs).m = _, congr,
+    exact D_set_move_eq_pos },
+  symmetry, change apply_A_move _ _ = _,
+  have h₁ : (play_D_move_at (init_game a d s) hs).s = s',
+  { convert h.symm, change apply_D_move s (d.f s hs).m = _,
+    congr, exact D_set_move_eq_pos },
+  congr' 1, change (a.f _ _ _).m = _, generalize_proofs h₂,
+  have h₃ : (a.f (play_D_move_at (init_game a d s) hs).s hs h₂).m =
+    (a.f s' hs₁ hvm_s').m, { congr' },
+  rw [h₃, A_set_move_eq_pos],
+end
+
+lemma A_hvm_of_next_act {pw : ℕ} {g : Game pw}
+  (h : g.play_move.act) :
+  ∃ hs, A_has_valid_move pw (play_D_move_at g hs).s.board :=
+begin
+  have hs : g.act := act_play_move_at_succ h, use hs,
+  rw Game.play_move at h, rw dif_pos hs at h,
+  rw play_A_move_at at h, split_ifs at h with h₄,
+  { cases h₄ with h₄ h₅, convert h₅, },
+  { cases h }
+end
+
+lemma play_move_hist_len_eq_of_act {pw : ℕ} {g : Game pw}
+  (h : g.play_move.act) :
+  g.play_move.s.len = g.s.len + 2 :=
+begin
+  have h₁ : g.act := act_play_move_at_succ h,
+  rw [play_move_at_act h₁, play_A_move_at],
+  rw dif_pos, { rw [hist_len_play_A_move_at', hist_len_play_D_move_at] },
+  exact ⟨h₁, (A_hvm_of_next_act h).some_spec⟩,
+end
+
+lemma play_hist_len_eq_of_act {pw n : ℕ} {g : Game pw}
+  (h : (g.play n).act) :
+  (g.play n).s.len = g.s.len + n * 2 :=
+begin
+  induction n with n ih, { refl }, rw play_at_succ' at h ⊢,
+  let g₁ : Game pw := _, change g.play n with g₁ at ih h ⊢,
+  have h₁ := act_play_move_at_succ h, specialize ih h₁,
+  rw [play_move_hist_len_eq_of_act h, ih, add_assoc, nat.succ_mul],
+end
+
+lemma hist_len_ne_of_play_lt {pw n k : ℕ} {g : Game pw}
+  (h₁ : k < n) (h₂ : (g.play n).act) :
+  (g.play k).s.len ≠ (g.play n).s.len :=
+begin
+  have h₃ := act_play_at_le (nat.le_of_lt h₁) h₂,
+  rw [play_hist_len_eq_of_act h₂, play_hist_len_eq_of_act h₃], intro h,
+  replace h := nat.add_left_cancel h,
+  rw nat.mul_left_inj at h, swap, { dec_trivial },
+  subst h, exact nat.lt_asymm h₁ h₁,
+end
+
+lemma hist_ne_of_play_lt {pw n k : ℕ} {g : Game pw}
+  (h₁ : k < n) (h₂ : (g.play n).act) :
+  (g.play k).s.history ≠ (g.play n).s.history :=
+hist_ne_of_hist_len_ne (hist_len_ne_of_play_lt h₁ h₂)
+
+lemma state_ne_of_play_lt {pw n k : ℕ} {g : Game pw}
+  (h₁ : k < n) (h₂ : (g.play n).act) :
+  (g.play k).s ≠ (g.play n).s :=
+by { have h₃ := hist_ne_of_play_lt h₁ h₂, contrapose! h₃, rw h₃ }
+
+lemma apply_A_move_ne_of_hist_ne {pw : ℕ} {s₁ s₂ : State}
+  {ma₁ ma₂ : A_move} (h : s₁.len ≠ s₂.len) :
+  apply_A_move s₁ ma₁ ≠ apply_A_move s₂ ma₂ :=
+begin
+  contrapose! h, simp_rw [apply_A_move, apply_move] at h,
+  simp_rw [State.len, (snoc_eq_snoc_iff.mp h.2.1).1],
+end
+
+lemma apply_D_move_ne_of_hist_ne {s₁ s₂ : State}
+  {md₁ md₂ : D_move} (h : s₁.len ≠ s₂.len) :
+  apply_D_move s₁ md₁ ≠ apply_D_move s₂ md₂ :=
+begin
+  contrapose! h, simp_rw [apply_D_move, apply_move] at h,
+  simp_rw [State.len, (snoc_eq_snoc_iff.mp h.2.1).1],
+end
+
+def mk_A_for_played_move_at_play_move {pw : ℕ}
+  (a₀ a : A pw) (s' : State) (hs : s'.act) :
+  A pw :=
+if hvm : A_has_valid_move pw s'.board
+then a₀.set_move s' (a.f s' hs hvm)
+else a₀
+
+lemma A_played_move_at_play_move {pw : ℕ}
+  {g : Game pw} {s₀' : State} {ma : Valid_A_move pw s₀'.board}
+  (h : A_played_move_at g.s s₀' ma) :
+  A_played_move_at g.play_move.s s₀' ma :=
+begin
+  let a := g.a, let d := g.d, let s := g.s,
+  rcases h with ⟨s₀, md₀, a₀, d₀, n, hmd, h₁, hx, hy, h₂⟩, by_cases hs : g.act,
+  { let md := d.f s hs, let s' := apply_D_move s md.m,
+    let d₁ := d₀.set_move s md,
+    let a₁ := mk_A_for_played_move_at_play_move a₀ a s' hs,
+    have hmd₁ : ∃ hs, d₁.f s₀ hs = md₀,
+    { cases hmd with hs₁ hmd, use hs₁, change dite _ _ _ = _,
+      rw dif_neg, { exact hmd }, change ((init_game a₀ d₀ s₀).play 0).s ≠ g.s,
+      rw h₂, apply state_ne_of_play_lt (nat.pos_of_ne_zero hy),
+      change g.s.act at hs, rwa h₂ at hs },
+    use [s₀, md₀, a₁, d₁, n.succ, hmd₁, by rw h₁],
+    have h₁ : ∀ (k ≤ n), ((init_game a₁ d₁ s₀).play k).s =
+      ((init_game a₀ d₀ s₀).play k).s,
+    { rintro k hk, induction k with k ih, { refl }, simp_rw play_at_succ',
+      specialize ih (nat.le_of_succ_le hk),
+      replace ih : (init_game a₁ d₁ s₀).play k =
+        ((init_game a₀ d₀ s₀).play k).set_players a₁ d₁,
+      { ext,
+        { exact play_at_players_eq.1 },
+        { exact play_at_players_eq.2 },
+        { rw ih, refl }},
+      rw ih, clear ih,
+      have hs₁ : ((init_game a₀ d₀ s₀).play k).act,
+      { apply act_play_at_le (nat.le_of_succ_le hk),
+        change ((init_game a₀ d₀ s₀).play n).s.act,
+        rw ←h₂, exact hs },
+      repeat { rw play_move_at_act, swap, { exact hs₁ }},
+      let g₁ : Game pw := _,
+      change (init_game a₀ d₀ s₀).play k with g₁ at hs₁ ⊢,
+      have ha : g₁.a = a₀ := play_at_players_eq.1,
+      have hd : g₁.d = d₀ := play_at_players_eq.2,
+      let sk := g₁.s, let mdk := d₀.f sk hs₁,
+      let sk' := apply_D_move sk mdk.m,
+      have hy : (play_D_move_at g₁ hs₁).s = sk',
+      { change apply_D_move sk _ = apply_D_move _ _, congr' 2, rw hd },
+      have h₁ : d₁.f sk hs₁ = mdk,
+      { change dite _ _ _ = _, rw dif_neg,
+        change ((init_game a₀ d₀ s₀).play k).s ≠ g.s, rw h₂,
+        apply state_ne_of_play_lt (nat.succ_le_iff.mp hk),
+        change ((init_game a₀ d₀ s₀).play n).s.act, rw ←h₂, exact hs },
+      have hx : play_D_move_at (g₁.set_players a₁ d₁) hs₁ =
+        (play_D_move_at g₁ hs₁).set_players a₁ d₁,
+      { ext,
+        { exact play_D_move_at_players_eq.1, },
+        { exact play_D_move_at_players_eq.2, },
+        { change apply_D_move g₁.s _ = apply_D_move _ _,
+          congr' 2, change d₁.f sk _ = _, rw [h₁, hd] }},
+      rw hx, clear hx, have hx : A_has_valid_move pw sk'.board,
+      { have h₃ : g₁.play_move.act,
+        { change ((init_game a₀ d₀ s₀).play k).play_move.act,
+          rw ←play_at_succ', apply act_play_at_le hk,
+          change ((init_game a₀ d₀ s₀).play n).s.act,
+          rw ←h₂, exact hs },
+        convert (A_hvm_of_next_act h₃).some_spec, rw ←hy, refl },
+      simp_rw play_A_move_at,
+      repeat { rw dif_pos, swap, { use hs₁, convert hx }},
+      change apply_A_move (play_D_move_at g₁ hs₁).s
+        (a₁.f (play_D_move_at g₁ hs₁).s _ _).m =
+        apply_A_move _ (g₁.a.f (play_D_move_at g₁ hs₁).s _ _).m,
+      congr' 2, rw ha, generalize_proofs h₃,
+      change (mk_A_for_played_move_at_play_move _ _ _ _).f _ _ _ = _,
+      rw mk_A_for_played_move_at_play_move,
+      split_ifs with hh, swap, { refl },
+      change dite _ _ _ = _, rw dif_neg, rw hy,
+      change apply_D_move ((init_game a₀ d₀ s₀).play k).s mdk.m ≠
+        apply_D_move g.s md.m,
+      rw h₂, replace hk := nat.lt_of_succ_le hk,
+      apply apply_D_move_ne_of_hist_ne, apply hist_len_ne_of_play_lt hk,
+      change ((init_game a₀ d₀ s₀).play n).s.act, rw ←h₂, exact hs },
+    specialize h₁ n (le_refl n),
+    replace h₁ : (init_game a₁ d₁ s₀).play n = g.set_players a₁ d₁,
+    { ext,
+      { exact play_at_players_eq.1 },
+      { exact play_at_players_eq.2 },
+      { rw h₁, exact h₂.symm }},
+    rw [play_at_succ', play_move_at_act hs, h₁, play_move_at_act],
+    swap, { exact hs }, refine ⟨_, _, _⟩,
+    { clear h₁, rcases hx with ⟨hs', h, hx⟩,
+      use [hs', h], rw ←hx, clear hx,
+      change (mk_A_for_played_move_at_play_move _ _ _ _).f _ _ _ = _,
+      rw mk_A_for_played_move_at_play_move,
+      split_ifs with hss, swap, { refl }, change dite _ _ _ = _,
+      rw dif_neg, change s₀' ≠ apply_D_move g.s _, rw [h₁, h₂],
+      apply apply_D_move_ne_of_hist_ne,
+      change ((init_game a₀ d₀ s₀).play 0).s.len ≠ _,
+      apply hist_len_ne_of_play_lt (pos_iff_ne_zero.mpr hy),
+      rw [Game.act, ←h₂], exact hs }, { dec_trivial }, symmetry,
+    have h₁ : play_D_move_at (g.set_players a₁ d₁) hs =
+      (play_D_move_at g hs).set_players a₁ d₁,
+    { ext,
+      { exact play_D_move_at_players_eq.1 },
+      { exact play_D_move_at_players_eq.2 },
+      { change apply_D_move g.s _ = apply_D_move _ _,
+        congr' 2, change d₁.f s hs = g.d.f g.s hs,
+        change dite _ _ _ = _, rw dif_pos rfl }},
+    rw h₁, clear h₁, simp_rw play_A_move_at,
+    split_ifs with h₁, swap, { refl }, cases h₁ with h₁ h₂,
+    change apply_A_move ((play_D_move_at g hs).s) _ =
+      apply_A_move _ _,
+    congr' 2, change a₁.f s' _ _ = a.f s' _ _, generalize_proofs,
+    change (mk_A_for_played_move_at_play_move _ _ _ _).f _ _ _ = _,
+    rw mk_A_for_played_move_at_play_move, rw dif_pos, swap, { exact h₂ },
+    change dite _ _ _ = _, rw dif_pos rfl },
+  { use [s₀, md₀, a₀, d₀, n, hmd, h₁, hx, hy],
+    rw play_move_at_not_act hs, exact h₂ },
+end
+
+lemma A_played_move_at_play {pw n : ℕ}
+  {g : Game pw} {s' : State} {ma : Valid_A_move pw s'.board}
+  (h : A_played_move_at g.s s' ma) :
+  A_played_move_at (g.play n).s s' ma :=
+begin
+  induction n with n ih, { exact h }, rw play_at_succ',
+  exact A_played_move_at_play_move ih,
+end
+
+lemma hist_overlaps_of_A_played_move_at {pw : ℕ}
+  {s s₀' : State} {ma : Valid_A_move pw s₀'.board}
+  (h₁ : A_played_move_at s s₀' ma) :
+  ∀ (k : ℕ), k.succ < s₀'.len →
+  s.history.nth k = s₀'.history.nth k :=
+begin
+  rintro k h₂,
+  rcases h₁ with ⟨s₀, md, a, d, n, hmd, rfl, hx, hy, rfl⟩, clear' hx hy,
+  change (apply_D_move s₀ md.m).history with (_ ++ _ : list _) at h₂ ⊢,
+  change _ < (snoc _ _).length at h₂,
+  rw [length_snoc, nat.succ_lt_succ_iff] at h₂ ,induction n with n ih,
+  { change s₀.history.nth k = _, exact (list.nth_append h₂).symm },
+  { simp_rw play_at_succ', let g : Game pw := _,
+    change (init_game a d s₀).play n with g at h₂ ih ⊢, rw ←ih, clear ih,
+    rw Game.play_move, split_ifs with hs, swap, { refl }, rw play_A_move_at,
+    have h₆ : s₀.len ≤ g.s.len,
+    { change (init_game a d s₀).s.len ≤ _, exact hist_len_le_play },
+    split_ifs with h₃,
+    { change (_ ++ _ : list _).nth _ = _, rw list.nth_append,
+      { change (_ ++ _ : list _).nth _ = _, rw list.nth_append,
+        exact gt_of_ge_of_gt h₆ h₂ },
+      { rw [←State.len, hist_len_play_D_move_at],
+        exact nat.lt_succ_of_le (nat.le_trans (le_of_lt h₂) h₆) }},
+    { change (_ ++ _ : list _).nth _ = _, rw list.nth_append,
+      exact gt_of_ge_of_gt h₆ h₂ }},
+end
+
+lemma A_played_move_at_eq_aux {pw n : ℕ}
+  {sx s₀ s' : State} {md : Valid_D_move s₀.board}
+  {a : A pw} {d : D} {hs hvm h₄}
+  (h₁ : s' = apply_D_move s₀ md.m)
+  (h₂ : sx = ((init_game a d s₀).play n).s)
+  (h₃ : n ≠ 0)
+  (hh : md = d.f s₀ h₄) :
+  sx.nth (s₀.len + 2) = option.some
+    (apply_A_move s' (a.f s' hs hvm).m).board :=
+begin
+  cases n, { contradiction }, clear h₃,
+  let i : ℕ := _, change s₀.len + 2 with i,
+  let s₁ : State := apply_A_move s' (a.f s' hs hvm).m,
+  change _ = some (State.board s₁), have h₅ : i = s₁.len,
+  { change s₁ with apply_A_move _ _, subst s',
+    rw [apply_A_move_len, apply_D_move_len] },
+  induction n with n ih generalizing sx,
+  { rw [play_1, play_move_at_act] at h₂, swap, { exact h₄ },
+    subst sx, have h₆ : play_D_move_at (init_game a d s₀) h₄ =
+      (init_game a d s'),
+    { ext,
+      { exact play_D_move_at_players_eq.1 },
+      { exact play_D_move_at_players_eq.2 },
+      { subst s',
+        change apply_D_move s₀ (d.f s₀ _).m = apply_D_move s₀ _, rw hh }},
+    rw [h₆, play_A_move_at, dif_pos], clear h₆, swap, { exact ⟨hs, hvm⟩ },
+    change s₁.nth _ = _, rw h₅, exact state_nth_len },
+  { rw play_at_succ' at h₂, let g₁ : Game pw := (init_game a d s₀).play n.succ,
+    change (init_game a d s₀).play n.succ with g₁ at ih h₂, subst sx,
+    specialize ih rfl, rw Game.play_move, split_ifs with hs₁, swap, { exact ih },
+    let g₂ : Game pw := _, change play_D_move_at g₁ hs₁ with g₂,
+    have ih₁ : g₂.s.nth i = some s₁.board,
+    { exact apply_move_state_nth_eq_some_of ih },
+    rw play_A_move_at, split_ifs with hh,
+    { exact apply_move_state_nth_eq_some_of ih₁ },
+    { exact ih₁ }},
+end
+
+lemma A_played_move_at_eq {pw : ℕ}
+  {sx s' : State} {ma₁ ma₂ : Valid_A_move pw s'.board}
+  (hx : A_played_move_at sx s' ma₁)
+  (hy : A_played_move_at sx s' ma₂) :
+  ma₁ = ma₂ :=
+begin
+  obtain ⟨s₀, md₁, a₁, d₁, n₁, hmd₁, h₁, ⟨hs₁, hvm₁, rfl⟩, h₃, h₄⟩ := hx,
+  obtain ⟨s₀', md₂, a₂, d₂, n₂, hmd₂, h₅, ⟨hs₂, hvm₂, rfl⟩, h₇, h₈⟩ := hy,
+  have hs : s₀.act,
+  { subst s', exact hs₂ },
+  obtain rfl : s₀ = s₀',
+  { subst h₁, exact state_eq_of_apply_D_move_eq h₅ },
+  obtain rfl : md₁ = md₂,
+  { subst h₁, rwa ←D_moves_eq_iff at h₅ },
+  clear h₅, change hvm₂ with hvm₁, clear hvm₂,
+  change hs₂ with hs₁, clear hs₂, let i := s₀.len,
+  have h₅ : sx.nth (i + 2) = option.some
+    (apply_A_move s' (a₁.f s' hs₁ hvm₁).m).board,
+  { exact A_played_move_at_eq_aux h₁ h₄ h₃ hmd₁.some_spec.symm },
+  have h₆ : sx.nth (i + 2) = option.some
+    (apply_A_move s' (a₂.f s' hs₁ hvm₁).m).board,
+  { exact A_played_move_at_eq_aux h₁ h₈ h₇ hmd₂.some_spec.symm },
+  simp [h₅] at h₆, rwa A_moves_eq_iff',
+end
